NuSys.thy
@@ -37,6 +37,7 @@ abbrevs
   and ">->" = "\<Zinj>"
   and "<;>" = "\<Zcomp>"
   and "<@GOAL>" = "\<^bold>@\<^bold>G\<^bold>O\<^bold>A\<^bold>L"
+  and "<val>" = "\<^bold>v\<^bold>a\<^bold>l"
 begin
 
 declare [ [ML_debugger, ML_exception_debugger] ]
@@ -63,13 +64,11 @@ ML_file NuHelp.ML
 subsection \<open>Code Block & Current Construction & Pending Construction\<close>
 
 definition (in std) CodeBlock :: "('RES_N \<Rightarrow> 'RES)
+                               \<Rightarrow> 'ret::value
                                \<Rightarrow> ('RES_N \<Rightarrow> 'RES)
-                               \<Rightarrow> ('VAL,'RES_N,'RES) M
-                               \<Rightarrow> ('FIC_N,'FIC) assn
-                               \<Rightarrow> ('FIC_N,'FIC) assn
+                               \<Rightarrow> ('ret,'RES_N,'RES) proc
                                \<Rightarrow> bool"
-  where "CodeBlock stat arg prog R E \<longleftrightarrow>
-             (bind arg prog = stat \<and> stat \<noteq> PartialCorrect \<and> (\<forall>s \<in> INTERP_COMP (R * E). stat \<noteq> Exception s))"
+  where "CodeBlock s' ret s prog \<longleftrightarrow> prog s = Success ret s' \<or> prog s = Fail"
 
 (* syntax "_codeblock_exp_" :: "idt \<Rightarrow> logic \<Rightarrow> logic \<Rightarrow> bool"  ("(2\<^bold>c\<^bold>o\<^bold>d\<^bold>e\<^bold>b\<^bold>l\<^bold>o\<^bold>c\<^bold>k _/  \<^bold>a\<^bold>s '\<open>_'\<close>/ \<^bold>f\<^bold>o\<^bold>r \<^bold>a\<^bold>r\<^bold>g\<^bold>u\<^bold>m\<^bold>e\<^bold>n\<^bold>t\<^bold>s '\<open>_'\<close>)" [100,0,0] 3)
 syntax "_codeblock_" :: "idt \<Rightarrow> logic \<Rightarrow> bool" ("\<^bold>c\<^bold>o\<^bold>d\<^bold>e\<^bold>b\<^bold>l\<^bold>o\<^bold>c\<^bold>k _ \<^bold>f\<^bold>o\<^bold>r \<^bold>a\<^bold>r\<^bold>g\<^bold>u\<^bold>m\<^bold>e\<^bold>n\<^bold>t\<^bold>s '\<open>_'\<close>" [100,0] 3) *)
@@ -81,13 +80,11 @@ definition (in std)
     ("\<^bold>c\<^bold>u\<^bold>r\<^bold>r\<^bold>e\<^bold>n\<^bold>t _ [_]/ \<^bold>r\<^bold>e\<^bold>s\<^bold>u\<^bold>l\<^bold>t\<^bold>s \<^bold>i\<^bold>n _" [1000,1000,11] 10)
   where "CurrentConstruction s R S \<longleftrightarrow> s \<in> (INTERP_COMP (R * S))"
 
-term bind
-
 definition (in std)
-  PendingConstruction :: " ('VAL,'RES_N,'RES) proc
+  PendingConstruction :: " ('ret::value,'RES_N,'RES) proc
                         \<Rightarrow> ('RES_N \<Rightarrow> 'RES)
                         \<Rightarrow> ('FIC_N,'FIC) assn
-                        \<Rightarrow> ('VAL list \<Rightarrow> ('FIC_N,'FIC) assn)
+                        \<Rightarrow> ('ret \<Rightarrow> ('FIC_N,'FIC) assn)
                         \<Rightarrow> ('FIC_N,'FIC) assn \<Rightarrow> bool "
     ("\<^bold>p\<^bold>e\<^bold>n\<^bold>d\<^bold>i\<^bold>n\<^bold>g _ \<^bold>o\<^bold>n _ [_]/ \<^bold>r\<^bold>e\<^bold>s\<^bold>u\<^bold>l\<^bold>t\<^bold>s \<^bold>i\<^bold>n _/ \<^bold>t\<^bold>h\<^bold>r\<^bold>o\<^bold>w\<^bold>s _" [1000,1000,1000,11,11] 10)
     where "PendingConstruction f s R S E \<longleftrightarrow> f s \<in> \<S> (\<lambda>ret. INTERP_COMP (R * S ret)) (INTERP_COMP (R * E))"
@@ -103,7 +100,7 @@ lemma (in std) CurrentConstruction_mk_elim_rule:
 
 paragraph \<open>Rules for Constructing Programs\<close>
 
-definition \<open>EMPTY_PROC = Success\<close>
+definition \<open>Return = Success\<close>
 
 context std begin
 
@@ -112,35 +109,21 @@ lemma \<phi>apply_proc:
   unfolding \<phi>Procedure_def CurrentConstruction_def PendingConstruction_def bind_def by (auto 0 5)
 
 lemma \<phi>accept_proc:
-  "\<^bold>p\<^bold>e\<^bold>n\<^bold>d\<^bold>i\<^bold>n\<^bold>g f \<^bold>o\<^bold>n s [R] \<^bold>r\<^bold>e\<^bold>s\<^bold>u\<^bold>l\<^bold>t\<^bold>s \<^bold>i\<^bold>n T \<^bold>t\<^bold>h\<^bold>r\<^bold>o\<^bold>w\<^bold>s E \<Longrightarrow> CodeBlock s' s f R E \<Longrightarrow> \<^bold>c\<^bold>u\<^bold>r\<^bold>r\<^bold>e\<^bold>n\<^bold>t s' [R] \<^bold>r\<^bold>e\<^bold>s\<^bold>u\<^bold>l\<^bold>t\<^bold>s \<^bold>i\<^bold>n T"
-  unfolding CurrentConstruction_def PendingConstruction_def CodeBlock_def
-  by (auto simp add: LooseStateTy_upgrade)
+  " \<^bold>p\<^bold>e\<^bold>n\<^bold>d\<^bold>i\<^bold>n\<^bold>g f \<^bold>o\<^bold>n s [R] \<^bold>r\<^bold>e\<^bold>s\<^bold>u\<^bold>l\<^bold>t\<^bold>s \<^bold>i\<^bold>n T \<^bold>t\<^bold>h\<^bold>r\<^bold>o\<^bold>w\<^bold>s E1
+\<Longrightarrow> (\<And>s' ret. \<^bold>c\<^bold>u\<^bold>r\<^bold>r\<^bold>e\<^bold>n\<^bold>t s' [R] \<^bold>r\<^bold>e\<^bold>s\<^bold>u\<^bold>l\<^bold>t\<^bold>s \<^bold>i\<^bold>n T ret \<Longrightarrow> \<^bold>p\<^bold>e\<^bold>n\<^bold>d\<^bold>i\<^bold>n\<^bold>g (g ret) \<^bold>o\<^bold>n s' [R] \<^bold>r\<^bold>e\<^bold>s\<^bold>u\<^bold>l\<^bold>t\<^bold>s \<^bold>i\<^bold>n U \<^bold>t\<^bold>h\<^bold>r\<^bold>o\<^bold>w\<^bold>s E2)
+\<Longrightarrow> \<^bold>p\<^bold>e\<^bold>n\<^bold>d\<^bold>i\<^bold>n\<^bold>g (f \<bind> g) \<^bold>o\<^bold>n s [R] \<^bold>r\<^bold>e\<^bold>s\<^bold>u\<^bold>l\<^bold>t\<^bold>s \<^bold>i\<^bold>n U \<^bold>t\<^bold>h\<^bold>r\<^bold>o\<^bold>w\<^bold>s E1 + E2"
+  unfolding CurrentConstruction_def PendingConstruction_def bind_def
+  by (cases "f s") (auto simp add: ring_distribs)
 
-lemma \<phi>reassemble_proc_0:
-  "\<^bold>c\<^bold>u\<^bold>r\<^bold>r\<^bold>e\<^bold>n\<^bold>t s [R] \<^bold>r\<^bold>e\<^bold>s\<^bold>u\<^bold>l\<^bold>t\<^bold>s \<^bold>i\<^bold>n T \<Longrightarrow> \<^bold>p\<^bold>e\<^bold>n\<^bold>d\<^bold>i\<^bold>n\<^bold>g EMPTY_PROC \<^bold>o\<^bold>n s [R] \<^bold>r\<^bold>e\<^bold>s\<^bold>u\<^bold>l\<^bold>t\<^bold>s \<^bold>i\<^bold>n T \<^bold>t\<^bold>h\<^bold>r\<^bold>o\<^bold>w\<^bold>s 0"
-  unfolding CurrentConstruction_def PendingConstruction_def CodeBlock_def bind_def EMPTY_PROC_def
-  by (cases s) simp+
-
-lemma \<phi>reassemble_proc:
-  " (\<And>s'. CodeBlock s' s f R E \<Longrightarrow> \<^bold>p\<^bold>e\<^bold>n\<^bold>d\<^bold>i\<^bold>n\<^bold>g g \<^bold>o\<^bold>n s' [R] \<^bold>r\<^bold>e\<^bold>s\<^bold>u\<^bold>l\<^bold>t\<^bold>s \<^bold>i\<^bold>n T \<^bold>t\<^bold>h\<^bold>r\<^bold>o\<^bold>w\<^bold>s E')
-\<Longrightarrow> \<^bold>p\<^bold>e\<^bold>n\<^bold>d\<^bold>i\<^bold>n\<^bold>g (f \<ggreater> g) \<^bold>o\<^bold>n s [R] \<^bold>r\<^bold>e\<^bold>s\<^bold>u\<^bold>l\<^bold>t\<^bold>s \<^bold>i\<^bold>n T \<^bold>t\<^bold>h\<^bold>r\<^bold>o\<^bold>w\<^bold>s E' + E"
-  unfolding CurrentConstruction_def PendingConstruction_def CodeBlock_def bind_def instr_comp_def
-            plus_set_def
-  apply auto
-  apply (meson INTERP_COMP_subset LooseStateTy_subset dual_order.refl in_mono inf_sup_ord(3) times_set_subset(1))
-  apply (metis (no_types, opaque_lifting) INTERP_COMP_subset subset_iff sup_ge1 sup_ge2 times_set_subset(1))
-  by (metis (no_types, lifting) INTERP_COMP_subset in_mono inf_sup_ord(3) inf_sup_ord(4) times_set_subset(1))
-
-lemma \<phi>reassemble_proc_00:
-  " (\<And>s'. CodeBlock s' s f R E \<Longrightarrow> \<^bold>p\<^bold>e\<^bold>n\<^bold>d\<^bold>i\<^bold>n\<^bold>g EMPTY_PROC \<^bold>o\<^bold>n s' [R] \<^bold>r\<^bold>e\<^bold>s\<^bold>u\<^bold>l\<^bold>t\<^bold>s \<^bold>i\<^bold>n T \<^bold>t\<^bold>h\<^bold>r\<^bold>o\<^bold>w\<^bold>s 0)
-\<Longrightarrow> \<^bold>p\<^bold>e\<^bold>n\<^bold>d\<^bold>i\<^bold>n\<^bold>g f \<^bold>o\<^bold>n s [R] \<^bold>r\<^bold>e\<^bold>s\<^bold>u\<^bold>l\<^bold>t\<^bold>s \<^bold>i\<^bold>n T \<^bold>t\<^bold>h\<^bold>r\<^bold>o\<^bold>w\<^bold>s E"
-  unfolding EMPTY_PROC_def
-  using \<phi>reassemble_proc[where E'=\<open>0\<close> and g = EMPTY_PROC, simplified EMPTY_PROC_def, simplified] .
+lemma \<phi>return:
+  "\<^bold>c\<^bold>u\<^bold>r\<^bold>r\<^bold>e\<^bold>n\<^bold>t s [R] \<^bold>r\<^bold>e\<^bold>s\<^bold>u\<^bold>l\<^bold>t\<^bold>s \<^bold>i\<^bold>n T ret \<Longrightarrow> \<^bold>p\<^bold>e\<^bold>n\<^bold>d\<^bold>i\<^bold>n\<^bold>g (Return ret) \<^bold>o\<^bold>n s [R] \<^bold>r\<^bold>e\<^bold>s\<^bold>u\<^bold>l\<^bold>t\<^bold>s \<^bold>i\<^bold>n T \<^bold>t\<^bold>h\<^bold>r\<^bold>o\<^bold>w\<^bold>s 0"
+  unfolding CurrentConstruction_def PendingConstruction_def CodeBlock_def bind_def Return_def
+  by simp+
 
 lemma \<phi>reassemble_proc_final:
   "(\<And>s H. \<^bold>c\<^bold>u\<^bold>r\<^bold>r\<^bold>e\<^bold>n\<^bold>t s [H] \<^bold>r\<^bold>e\<^bold>s\<^bold>u\<^bold>l\<^bold>t\<^bold>s \<^bold>i\<^bold>n S \<Longrightarrow> \<^bold>p\<^bold>e\<^bold>n\<^bold>d\<^bold>i\<^bold>n\<^bold>g g \<^bold>o\<^bold>n s [H] \<^bold>r\<^bold>e\<^bold>s\<^bold>u\<^bold>l\<^bold>t\<^bold>s \<^bold>i\<^bold>n T \<^bold>t\<^bold>h\<^bold>r\<^bold>o\<^bold>w\<^bold>s E) \<Longrightarrow> \<^bold>p\<^bold>r\<^bold>o\<^bold>c g \<lbrace> S \<longmapsto> T \<^bold>t\<^bold>h\<^bold>r\<^bold>o\<^bold>w\<^bold>s E\<rbrace>"
   unfolding CurrentConstruction_def PendingConstruction_def \<phi>Procedure_def bind_def pair_All
-  by (metis StrictStateTy_intro(1) state.simps(15))
+  by blast
 
 
 lemma \<phi>rename_proc: "f \<equiv> f' \<Longrightarrow> \<^bold>p\<^bold>r\<^bold>o\<^bold>c f' \<lbrace> U \<longmapsto> \<R> \<^bold>t\<^bold>h\<^bold>r\<^bold>o\<^bold>w\<^bold>s E \<rbrace> \<Longrightarrow> \<^bold>p\<^bold>r\<^bold>o\<^bold>c f \<lbrace> U \<longmapsto> \<R> \<^bold>t\<^bold>h\<^bold>r\<^bold>o\<^bold>w\<^bold>s E \<rbrace>" by fast
@@ -383,9 +366,10 @@ lemma \<phi>Type_eqI:
 paragraph \<open>Syntax\<close>
 
 abbreviation (in std) COMMA
-  :: \<open>('VAL,'FIC_N,'FIC) comp set \<Rightarrow> ('VAL,'FIC_N,'FIC) comp set \<Rightarrow> ('VAL,'FIC_N,'FIC) comp set\<close> (infixl "\<heavy_comma>" 13)
+  :: \<open>('FIC_N,'FIC) assn \<Rightarrow> ('FIC_N,'FIC) assn \<Rightarrow> ('FIC_N,'FIC) assn\<close> (infixl "\<heavy_comma>" 13)
   where \<open>COMMA \<equiv> (*)\<close>
 
+(*
 setup \<open>(Sign.add_trrules (let open Ast 
       fun nuty x y = Appl [Constant \<^const_syntax>\<open>\<phi>Type\<close>, Variable x, Variable y]
       fun wrap_ele tm = Appl [Constant \<^const_syntax>\<open>Ele\<close>, tm]
@@ -416,7 +400,7 @@ setup \<open>(Sign.add_trrules (let open Ast
         Appl [Constant "\<^const>local.PendingConstruction", Variable "f", Variable "s", Variable "R", nuty "x" "T"],
         Appl [Constant "\<^const>local.PendingConstruction", Variable "f", Variable "s", Variable "R", wrap_nuty "x" "T"])
   ] end))\<close>
-
+*)
 
 subsubsection \<open>Properties\<close>
 
@@ -443,19 +427,19 @@ definition Subty :: " 'a set \<Rightarrow> 'a set \<Rightarrow> bool \<Rightarro
 
 lemma (in std) \<phi>CONSEQ':
    "\<^bold>s\<^bold>u\<^bold>b\<^bold>t\<^bold>y\<^bold>p\<^bold>e A' \<longmapsto> A \<^bold>w\<^bold>i\<^bold>t\<^bold>h P1
-\<Longrightarrow> \<^bold>s\<^bold>u\<^bold>b\<^bold>t\<^bold>y\<^bold>p\<^bold>e B \<longmapsto> B' \<^bold>w\<^bold>i\<^bold>t\<^bold>h P2
+\<Longrightarrow> (\<And>x. \<^bold>s\<^bold>u\<^bold>b\<^bold>t\<^bold>y\<^bold>p\<^bold>e B x \<longmapsto> B' x \<^bold>w\<^bold>i\<^bold>t\<^bold>h P2)
 \<Longrightarrow> \<^bold>s\<^bold>u\<^bold>b\<^bold>t\<^bold>y\<^bold>p\<^bold>e E \<longmapsto> E' \<^bold>w\<^bold>i\<^bold>t\<^bold>h P3
 \<Longrightarrow> \<^bold>p\<^bold>r\<^bold>o\<^bold>c f \<lbrace> A  \<longmapsto> B  \<^bold>t\<^bold>h\<^bold>r\<^bold>o\<^bold>w\<^bold>s E  \<rbrace>
 \<Longrightarrow> \<^bold>p\<^bold>r\<^bold>o\<^bold>c f \<lbrace> A' \<longmapsto> B' \<^bold>t\<^bold>h\<^bold>r\<^bold>o\<^bold>w\<^bold>s E' \<rbrace>"
   unfolding Subty_def
-  using \<phi>CONSEQ[unfolded subset_iff] by simp
+  by (meson \<phi>CONSEQ subsetI)
 
 lemma (in std) \<phi>CONSEQ'E:
    "\<^bold>s\<^bold>u\<^bold>b\<^bold>t\<^bold>y\<^bold>p\<^bold>e E \<longmapsto> E' \<^bold>w\<^bold>i\<^bold>t\<^bold>h P3
 \<Longrightarrow> \<^bold>p\<^bold>r\<^bold>o\<^bold>c f \<lbrace> A  \<longmapsto> B  \<^bold>t\<^bold>h\<^bold>r\<^bold>o\<^bold>w\<^bold>s E  \<rbrace>
 \<Longrightarrow> \<^bold>p\<^bold>r\<^bold>o\<^bold>c f \<lbrace> A \<longmapsto> B \<^bold>t\<^bold>h\<^bold>r\<^bold>o\<^bold>w\<^bold>s E' \<rbrace>"
   unfolding Subty_def
-  using \<phi>CONSEQ[unfolded subset_iff] by simp
+  by (meson \<phi>CONSEQ subsetI)
 
 subsubsection \<open>Subjection\<close>
 
@@ -477,8 +461,8 @@ lemma [\<phi>reason]:
   unfolding Subty_def Premise_def by (simp add: \<phi>expns)
 
 lemma [simp]: "(T \<^bold>s\<^bold>u\<^bold>b\<^bold>j True) = T" by (auto simp add: \<phi>expns)
-lemma (in std) [simp]: "(VAL (S \<^bold>s\<^bold>u\<^bold>b\<^bold>j P)) = (VAL S \<^bold>s\<^bold>u\<^bold>b\<^bold>j P)" by (simp add: \<phi>expns set_eq_iff) blast
-lemma (in std) [simp]: "(OBJ (S \<^bold>s\<^bold>u\<^bold>b\<^bold>j P)) = (OBJ S \<^bold>s\<^bold>u\<^bold>b\<^bold>j P)" by (simp add: \<phi>expns set_eq_iff)
+(* lemma (in std) [simp]: "(VAL (S \<^bold>s\<^bold>u\<^bold>b\<^bold>j P)) = (VAL S \<^bold>s\<^bold>u\<^bold>b\<^bold>j P)" by (simp add: \<phi>expns set_eq_iff) blast
+lemma (in std) [simp]: "(OBJ (S \<^bold>s\<^bold>u\<^bold>b\<^bold>j P)) = (OBJ S \<^bold>s\<^bold>u\<^bold>b\<^bold>j P)" by (simp add: \<phi>expns set_eq_iff) *)
 
 lemma Subjection_times[simp]:
   \<open>(S \<^bold>s\<^bold>u\<^bold>b\<^bold>j P) * T = (S * T \<^bold>s\<^bold>u\<^bold>b\<^bold>j P)\<close>
@@ -489,7 +473,7 @@ lemma Subjection_times[simp]:
 (* declare split_paired_All[simp del] split_paired_Ex[simp del] *)
 
 lemma (in std) Subjection_simp_proc_arg'[simp]:
-  "\<^bold>p\<^bold>r\<^bold>o\<^bold>c f \<lbrace> T \<^bold>s\<^bold>u\<^bold>b\<^bold>j P \<longmapsto> Y \<rbrace> = (P \<longrightarrow> \<^bold>p\<^bold>r\<^bold>o\<^bold>c f \<lbrace> T \<longmapsto> Y \<rbrace>)"
+  "\<^bold>p\<^bold>r\<^bold>o\<^bold>c f \<lbrace> T \<^bold>s\<^bold>u\<^bold>b\<^bold>j P \<longmapsto> Y \<^bold>t\<^bold>h\<^bold>r\<^bold>o\<^bold>w\<^bold>s E \<rbrace> = (P \<longrightarrow> \<^bold>p\<^bold>r\<^bold>o\<^bold>c f \<lbrace> T \<longmapsto> Y \<^bold>t\<^bold>h\<^bold>r\<^bold>o\<^bold>w\<^bold>s E \<rbrace>)"
   (* and Subjection_simp_func_arg[simp]: "\<^bold>f\<^bold>u\<^bold>n\<^bold>c f' \<lbrace> T \<and>\<^sup>s P \<longmapsto> Y \<rbrace> = (P \<longrightarrow> \<^bold>f\<^bold>u\<^bold>n\<^bold>c f' \<lbrace> T \<longmapsto> Y \<rbrace>)" *)
   unfolding \<phi>Procedure_def by (simp add: \<phi>expns) blast
 
@@ -497,14 +481,14 @@ lemmas (in std) Subjection_simp_proc_arg[unfolded atomize_eq[symmetric]] = Subje
 
 lemma (in std) [simp]:
   "(\<^bold>c\<^bold>u\<^bold>r\<^bold>r\<^bold>e\<^bold>n\<^bold>t s [H] \<^bold>r\<^bold>e\<^bold>s\<^bold>u\<^bold>l\<^bold>t\<^bold>s \<^bold>i\<^bold>n T \<^bold>s\<^bold>u\<^bold>b\<^bold>j P) \<longleftrightarrow> (\<^bold>c\<^bold>u\<^bold>r\<^bold>r\<^bold>e\<^bold>n\<^bold>t s [H] \<^bold>r\<^bold>e\<^bold>s\<^bold>u\<^bold>l\<^bold>t\<^bold>s \<^bold>i\<^bold>n T) \<and> P"
-  unfolding CurrentConstruction_def by (cases s, simp_all add: \<phi>expns pair_All) blast
+  unfolding CurrentConstruction_def by (simp_all add: \<phi>expns pair_All) blast
 
 lemma (in std) [simp]:
   "((\<^bold>c\<^bold>u\<^bold>r\<^bold>r\<^bold>e\<^bold>n\<^bold>t s [H] \<^bold>r\<^bold>e\<^bold>s\<^bold>u\<^bold>l\<^bold>t\<^bold>s \<^bold>i\<^bold>n T) \<and> B) \<and> C \<longleftrightarrow> (\<^bold>c\<^bold>u\<^bold>r\<^bold>r\<^bold>e\<^bold>n\<^bold>t s [H] \<^bold>r\<^bold>e\<^bold>s\<^bold>u\<^bold>l\<^bold>t\<^bold>s \<^bold>i\<^bold>n T) \<and> (B \<and> C)"
   by simp
 
 
-ML \<open>Theory.setup (Sign.add_trrules (let open Ast 
+(* ML \<open>Theory.setup (Sign.add_trrules (let open Ast 
       fun nuty x y = Appl [Constant \<^const_syntax>\<open>\<phi>Type\<close>, Variable x, Variable y]
       fun wrap_ele tm = Appl [Constant \<^const_syntax>\<open>Ele\<close>, tm]
       fun wrap_nuty x y = wrap_ele (nuty x y)
@@ -523,7 +507,7 @@ ML \<open>Theory.setup (Sign.add_trrules (let open Ast
         Appl [Constant "\<^const>local.\<phi>Procedure_no_exception", Variable "f", Variable "U", subj (nuty "x" "T")],
         Appl [Constant "\<^const>local.\<phi>Procedure_no_exception", Variable "f", Variable "U", subj (wrap_nuty "x" "T")])
   ] end))\<close>
-
+*)
 
 
 subsubsection \<open>Existential Quantification\<close>
@@ -536,13 +520,14 @@ notation ExSet (binder "\<exists>\<^sup>s" 10)
 lemma [\<phi>expns]: "p \<in> ExSet S \<longleftrightarrow> (\<exists>c. p \<in> S c)" unfolding ExSet_def by simp
 
 syntax
-  "_SetcomprNu" :: "'a \<Rightarrow> idts \<Rightarrow> bool \<Rightarrow> 'a set"  ("_ \<^bold>s\<^bold>u\<^bold>b\<^bold>j/ _./ _" [2,0,3] 2)
+  "_SetcomprNu" :: "'a \<Rightarrow> idts \<Rightarrow> bool \<Rightarrow> 'a set"  ("_ \<^bold>s\<^bold>u\<^bold>b\<^bold>j/ _./ _" [3,0,4] 3)
 
 translations
   " X \<^bold>s\<^bold>u\<^bold>b\<^bold>j idts. P " \<rightleftharpoons> "\<exists>* idts. X \<^bold>s\<^bold>u\<^bold>b\<^bold>j P"
   " X \<^bold>s\<^bold>u\<^bold>b\<^bold>j idts. CONST True " \<rightleftharpoons> "\<exists>* idts. X"
 
 
+(*
 ML \<open>Theory.setup (Sign.add_trrules (let open Ast 
       fun nuty x y = Appl [Constant \<^const_syntax>\<open>\<phi>Type\<close>, Variable x, Variable y]
       fun wrap_ele tm = Appl [Constant \<^const_syntax>\<open>Ele\<close>, tm]
@@ -562,9 +547,9 @@ ML \<open>Theory.setup (Sign.add_trrules (let open Ast
         Appl [Constant "\<^const>local.\<phi>Procedure_no_exception", Variable "f", Variable "U", subj (nuty "x" "T")],
         Appl [Constant "\<^const>local.\<phi>Procedure_no_exception", Variable "f", Variable "U", subj (wrap_nuty "x" "T")])
   ] end))\<close>
-
+*)
 text (in std)
- \<open>The set of \<phi>-type in an assertion like \<^term>\<open>\<^bold>p\<^bold>r\<^bold>o\<^bold>c f \<lbrace> S x \<^bold>s\<^bold>u\<^bold>b\<^bold>j x. P x \<longmapsto> T x \<^bold>s\<^bold>u\<^bold>b\<^bold>j x. Q x \<rbrace>\<close> is represented
+ \<open>The set of \<phi>-type in an assertion like \<^term>\<open>\<^bold>p\<^bold>r\<^bold>o\<^bold>c f \<lbrace> S x \<^bold>s\<^bold>u\<^bold>b\<^bold>j x. P x \<longmapsto> \<lambda>ret. T x \<^bold>s\<^bold>u\<^bold>b\<^bold>j x. Q x \<rbrace>\<close> is represented
   by \<^const>\<open>ExSet\<close> and we show a \<phi>-type \<^term>\<open>S x \<^bold>s\<^bold>u\<^bold>b\<^bold>j x. P x\<close> represents actually all concrete values that
   belongs to \<^term>\<open>S\<close> a set of \<phi>-types (i.e. the union of \<^term>\<open>S\<close>) by following lemma\<close>
 
@@ -577,8 +562,8 @@ lemma named_ExSet: "(ExSet T) = (\<exists>*c. T (tag c) )" by (auto simp add: na
 
 (* lemma (in std_sem) [simp]: "p \<in> \<S>  (ExSet T) \<longleftrightarrow> (\<exists>z. p \<in> \<S>  (T z) )" by (cases p, simp_all add: \<phi>expns set_eq_iff)
 lemma (in std_sem) [simp]: "p \<in> !\<S> (ExSet T) \<longleftrightarrow> (\<exists>z. p \<in> !\<S> (T z) )" by (cases p, simp_all add: \<phi>expns set_eq_iff) *)
-lemma (in std) [simp]: "(VAL ExSet T) = (\<exists>*c. VAL T c)" by (simp add: \<phi>expns set_eq_iff) blast
-lemma (in std) [simp]: "(OBJ ExSet T) = (\<exists>*c. OBJ T c)" by (simp add: \<phi>expns set_eq_iff)
+(* lemma (in std) [simp]: "(VAL ExSet T) = (\<exists>*c. VAL T c)" by (simp add: \<phi>expns set_eq_iff) blast
+lemma (in std) [simp]: "(OBJ ExSet T) = (\<exists>*c. OBJ T c)" by (simp add: \<phi>expns set_eq_iff) *)
 lemma [simp]: "(ExSet T * R) = (\<exists>* c. T c * R )" by (simp add: \<phi>expns set_eq_iff) blast
 lemma ExSet_times[simp]: "(L * ExSet T) = (\<exists>* c. L * T c)" by (simp add: \<phi>expns set_eq_iff) blast
 
@@ -593,11 +578,10 @@ lemma ExSet_SubjSet[simp]:
 
 lemma (in std) \<phi>ExTyp_strip:
   "(\<^bold>c\<^bold>u\<^bold>r\<^bold>r\<^bold>e\<^bold>n\<^bold>t p [H] \<^bold>r\<^bold>e\<^bold>s\<^bold>u\<^bold>l\<^bold>t\<^bold>s \<^bold>i\<^bold>n (ExSet T)) \<equiv> (\<exists>c. \<^bold>c\<^bold>u\<^bold>r\<^bold>r\<^bold>e\<^bold>n\<^bold>t p [H] \<^bold>r\<^bold>e\<^bold>s\<^bold>u\<^bold>l\<^bold>t\<^bold>s \<^bold>i\<^bold>n T c)"
-  unfolding CurrentConstruction_def atomize_eq by (cases p, simp_all add: \<phi>expns pair_All) blast
+  unfolding CurrentConstruction_def atomize_eq by (simp_all add: \<phi>expns pair_All) blast
 
 lemma [\<phi>reason 200]: "(\<And>c. \<^bold>s\<^bold>u\<^bold>b\<^bold>t\<^bold>y\<^bold>p\<^bold>e T c \<longmapsto> T' \<^bold>w\<^bold>i\<^bold>t\<^bold>h P c) \<Longrightarrow> \<^bold>s\<^bold>u\<^bold>b\<^bold>t\<^bold>y\<^bold>p\<^bold>e (ExSet T) \<longmapsto> T' \<^bold>w\<^bold>i\<^bold>t\<^bold>h (\<exists>c. P c)"
   unfolding Subty_def by (simp add: \<phi>expns) blast
-
 
 
 
@@ -633,8 +617,6 @@ subsubsection \<open>Reasoning Rules & Settings\<close>
 declare set_mult_inhabited[\<phi>reason_elim!]
   Premise_def[\<phi>def, \<phi>expns]
 
-declare (in std) Obj_Ele_inhabited[\<phi>reason_elim!] Val_Ele_inhabited[\<phi>reason_elim!]
-
 lemma (in std) [\<phi>reason]:
   \<open> (\<And>x. \<phi>SemType (x \<Ztypecolon> T) TY)
 \<Longrightarrow> \<phi>\<phi>SemType T TY\<close>
@@ -646,7 +628,7 @@ lemma (in std) [\<phi>reason_elim!, elim!]:
 
 subsubsection \<open>Finalization Rewrites\<close>
 
-lemmas final_proc_rewrite = proc_bind_SKIP[folded EMPTY_PROC_def]
+lemmas final_proc_rewrite = ""
 
 
 subsection \<open>Ad-hoc Overload\<close>
@@ -720,28 +702,12 @@ lemma \<phi>cast_intro_frame_R:
 lemma (in std) "\<phi>cast":
   "\<^bold>c\<^bold>u\<^bold>r\<^bold>r\<^bold>e\<^bold>n\<^bold>t blk [H] \<^bold>r\<^bold>e\<^bold>s\<^bold>u\<^bold>l\<^bold>t\<^bold>s \<^bold>i\<^bold>n T \<Longrightarrow> \<^bold>s\<^bold>u\<^bold>b\<^bold>t\<^bold>y\<^bold>p\<^bold>e T \<longmapsto> T' \<^bold>w\<^bold>i\<^bold>t\<^bold>h P \<Longrightarrow> \<^bold>c\<^bold>u\<^bold>r\<^bold>r\<^bold>e\<^bold>n\<^bold>t blk [H] \<^bold>r\<^bold>e\<^bold>s\<^bold>u\<^bold>l\<^bold>t\<^bold>s \<^bold>i\<^bold>n T'"
   unfolding CurrentConstruction_def Subty_def
-  by (cases blk, simp_all add: pair_All \<phi>expns) blast
+  by (simp_all add: pair_All \<phi>expns) blast
 
 lemma (in std) "\<phi>cast_P":
   "\<^bold>c\<^bold>u\<^bold>r\<^bold>r\<^bold>e\<^bold>n\<^bold>t blk [H] \<^bold>r\<^bold>e\<^bold>s\<^bold>u\<^bold>l\<^bold>t\<^bold>s \<^bold>i\<^bold>n T \<Longrightarrow> \<^bold>s\<^bold>u\<^bold>b\<^bold>t\<^bold>y\<^bold>p\<^bold>e T \<longmapsto> T' \<^bold>w\<^bold>i\<^bold>t\<^bold>h P \<Longrightarrow> (\<^bold>c\<^bold>u\<^bold>r\<^bold>r\<^bold>e\<^bold>n\<^bold>t blk [H] \<^bold>r\<^bold>e\<^bold>s\<^bold>u\<^bold>l\<^bold>t\<^bold>s \<^bold>i\<^bold>n T') \<and> P"
   unfolding CurrentConstruction_def Subty_def
-  by (cases blk, simp_all add: pair_All \<phi>expns) blast
-
-lemma (in std) cast_val_\<phi>app[\<phi>overload cast]:
-  "\<^bold>a\<^bold>r\<^bold>g\<^bold>u\<^bold>m\<^bold>e\<^bold>n\<^bold>t \<^bold>s\<^bold>u\<^bold>b\<^bold>t\<^bold>y\<^bold>p\<^bold>e X \<longmapsto> X' \<^bold>w\<^bold>i\<^bold>t\<^bold>h P \<Longrightarrow> \<^bold>s\<^bold>u\<^bold>b\<^bold>t\<^bold>y\<^bold>p\<^bold>e (VAL X) \<longmapsto> VAL X' \<^bold>w\<^bold>i\<^bold>t\<^bold>h P"
-  unfolding Subty_def Argument_def
-  by (simp_all add: \<phi>expns, blast)
-
-lemma (in std) cast_vals_\<phi>app:
-  "\<^bold>a\<^bold>r\<^bold>g\<^bold>u\<^bold>m\<^bold>e\<^bold>n\<^bold>t \<^bold>s\<^bold>u\<^bold>b\<^bold>t\<^bold>y\<^bold>p\<^bold>e VAL X \<longmapsto> XX \<^bold>w\<^bold>i\<^bold>t\<^bold>h P \<Longrightarrow> \<^bold>s\<^bold>u\<^bold>b\<^bold>t\<^bold>y\<^bold>p\<^bold>e (VAL X) \<longmapsto> XX \<^bold>w\<^bold>i\<^bold>t\<^bold>h P"
-  unfolding Subty_def Argument_def
-  by (simp_all add: \<phi>expns)
-
-lemma (in std) cast_objs_\<phi>app:
-  "\<^bold>a\<^bold>r\<^bold>g\<^bold>u\<^bold>m\<^bold>e\<^bold>n\<^bold>t \<^bold>s\<^bold>u\<^bold>b\<^bold>t\<^bold>y\<^bold>p\<^bold>e OBJ Y \<longmapsto> YY \<^bold>w\<^bold>i\<^bold>t\<^bold>h P \<Longrightarrow> \<^bold>s\<^bold>u\<^bold>b\<^bold>t\<^bold>y\<^bold>p\<^bold>e (OBJ Y) \<longmapsto> YY \<^bold>w\<^bold>i\<^bold>t\<^bold>h P"
-  unfolding Subty_def Argument_def
-  by (simp_all add: \<phi>expns, blast)
-
+  by (simp_all add: pair_All \<phi>expns) blast
 
 lemma cast_whole_\<phi>app:
   "\<^bold>a\<^bold>r\<^bold>g\<^bold>u\<^bold>m\<^bold>e\<^bold>n\<^bold>t \<^bold>s\<^bold>u\<^bold>b\<^bold>t\<^bold>y\<^bold>p\<^bold>e X \<longmapsto> X' \<^bold>w\<^bold>i\<^bold>t\<^bold>h P \<Longrightarrow> \<^bold>s\<^bold>u\<^bold>b\<^bold>t\<^bold>y\<^bold>p\<^bold>e X \<longmapsto> X' \<^bold>w\<^bold>i\<^bold>t\<^bold>h P"
@@ -768,28 +734,47 @@ consts frame_var_rewrs :: mode
 context std begin
 
 definition IntroFrameVar ::
-  "('VAL,'FIC_N,'FIC) assn
-\<Rightarrow> ('VAL,'FIC_N,'FIC) assn \<Rightarrow> ('VAL,'FIC_N,'FIC) assn
-\<Rightarrow> ('VAL,'FIC_N,'FIC) assn \<Rightarrow> ('VAL,'FIC_N,'FIC) assn
-\<Rightarrow> ('VAL,'FIC_N,'FIC) assn \<Rightarrow> ('VAL,'FIC_N,'FIC) assn
+  "('FIC_N,'FIC) assn
+\<Rightarrow> ('FIC_N,'FIC) assn \<Rightarrow> ('FIC_N,'FIC) assn
+\<Rightarrow> ('FIC_N,'FIC) assn \<Rightarrow> ('FIC_N,'FIC) assn
 \<Rightarrow> bool"
-  where "IntroFrameVar R S' S T' T E' E \<longleftrightarrow> S' = (R * S) \<and> T' = (R * T) \<and> E' = (R * E) "
+  where "IntroFrameVar R S' S T' T \<longleftrightarrow> S' = (R * S) \<and> T' = R * T "
+
+definition IntroFrameVar' ::
+  "('FIC_N,'FIC) assn
+\<Rightarrow> ('FIC_N,'FIC) assn \<Rightarrow> ('FIC_N,'FIC) assn
+\<Rightarrow> ('ret \<Rightarrow> ('FIC_N,'FIC) assn) \<Rightarrow> ('ret \<Rightarrow> ('FIC_N,'FIC) assn)
+\<Rightarrow> ('FIC_N,'FIC) assn \<Rightarrow> ('FIC_N,'FIC) assn
+\<Rightarrow> bool"
+  where "IntroFrameVar' R S' S T' T E' E \<longleftrightarrow> S' = (R * S) \<and> T' = (\<lambda>ret. R * T ret) \<and> E' = (R * E) "
+
 
 lemma IntroFrameVar_No:
-  "IntroFrameVar Void S S T T E E"
+  "IntroFrameVar Void S S T T"
   unfolding IntroFrameVar_def by simp
+
+lemma IntroFrameVar'_No:
+  "IntroFrameVar' Void S S T T E E"
+  unfolding IntroFrameVar'_def by simp
 
 lemma IntroFrameVar_Yes:
   " Simplify frame_var_rewrs S' (R * S)
 \<Longrightarrow> Simplify frame_var_rewrs T' (R * T)
-\<Longrightarrow> Simplify frame_var_rewrs E' (R * E)
-\<Longrightarrow> IntroFrameVar R S' S T' T E' E"
+\<Longrightarrow> IntroFrameVar R S' S T' T"
   unfolding IntroFrameVar_def by blast
 
-\<phi>reasoner_ML IntroFrameVar 1000 (conclusion "IntroFrameVar ?R ?S' ?S ?T' ?T ?E' ?E") =
+lemma IntroFrameVar'_Yes:
+  " Simplify frame_var_rewrs S' (R * S)
+\<Longrightarrow> Simplify frame_var_rewrs T' (\<lambda>ret. R * T ret)
+\<Longrightarrow> Simplify frame_var_rewrs E' (R * E)
+\<Longrightarrow> IntroFrameVar' R S' S T' T E' E"
+  unfolding IntroFrameVar'_def by blast
+
+
+\<phi>reasoner_ML IntroFrameVar 1000 (conclusion "IntroFrameVar ?R ?S' ?S ?T' ?T") =
 \<open>fn (ctxt, sequent) =>
   let
-    val (Const (\<^const_name>\<open>std.IntroFrameVar\<close>, _) $ _ $ _ $ S $ _ $ _ $ _ $ _) =
+    val (Const (\<^const_name>\<open>std.IntroFrameVar\<close>, _) $ _ $ _ $ S $ _ $ _) =
         Thm.major_prem_of sequent |> HOLogic.dest_Trueprop
     val tail = PhiSyntax.strip_separations S |> NuHelp.last
   in
@@ -797,6 +782,19 @@ lemma IntroFrameVar_Yes:
     then Seq.single (ctxt, @{thm IntroFrameVar_No} RS sequent)
     else Seq.single (ctxt, @{thm IntroFrameVar_Yes} RS sequent)
   end\<close>
+
+\<phi>reasoner_ML IntroFrameVar' 1000 (conclusion "IntroFrameVar' ?R ?S' ?S ?T' ?T ?E' ?E") =
+\<open>fn (ctxt, sequent) =>
+  let
+    val (Const (\<^const_name>\<open>std.IntroFrameVar'\<close>, _) $ _ $ _ $ S $ _ $ _ $ _ $ _) =
+        Thm.major_prem_of sequent |> HOLogic.dest_Trueprop
+    val tail = PhiSyntax.strip_separations S |> NuHelp.last
+  in
+    if is_Var tail andalso fastype_of tail = PhiSyntax.get_assn_typ ctxt
+    then Seq.single (ctxt, @{thm IntroFrameVar'_No} RS sequent)
+    else Seq.single (ctxt, @{thm IntroFrameVar'_Yes} RS sequent)
+  end\<close>
+
 
 end
 
@@ -821,16 +819,14 @@ text (in std) \<open>During the subtyping reasoning, \<^term>\<open>FIX OBJ S\<c
   and fixed. For example, a cast may apply only on the first object,
   after user rotates the target to the first.\<close>
 
-translations "FIX (x \<Ztypecolon> T)" \<rightleftharpoons> "FIX ELE (x \<Ztypecolon> T)"
-
 lemma [\<phi>reason 2000]:
   \<open>\<^bold>s\<^bold>u\<^bold>b\<^bold>t\<^bold>y\<^bold>p\<^bold>e X \<longmapsto> Y \<^bold>w\<^bold>i\<^bold>t\<^bold>h P \<Longrightarrow> \<^bold>s\<^bold>u\<^bold>b\<^bold>t\<^bold>y\<^bold>p\<^bold>e X \<longmapsto> FIX Y \<^bold>w\<^bold>i\<^bold>t\<^bold>h P\<close>
   unfolding Fix_def .
 
-lemma (in std) cast_obj_\<phi>app:
+(* lemma (in std) cast_obj_\<phi>app:
   "\<^bold>a\<^bold>r\<^bold>g\<^bold>u\<^bold>m\<^bold>e\<^bold>n\<^bold>t \<^bold>s\<^bold>u\<^bold>b\<^bold>t\<^bold>y\<^bold>p\<^bold>e Y \<longmapsto> Y' \<^bold>w\<^bold>i\<^bold>t\<^bold>h P \<Longrightarrow> \<^bold>s\<^bold>u\<^bold>b\<^bold>t\<^bold>y\<^bold>p\<^bold>e (FIX OBJ Y) \<longmapsto> OBJ Y' \<^bold>w\<^bold>i\<^bold>t\<^bold>h P"
   unfolding Subty_def Argument_def Fix_def
-  by (simp_all add: \<phi>expns, blast)
+  by (simp_all add: \<phi>expns, blast) *)
 
 
 
@@ -879,24 +875,22 @@ text (in std) \<open>
   SYNTHESIS tags a part of the post \<phi>-type of a triple, representing this part is synthesised
     by the procedure of this triple. The procedure generates some values (or state) that meet
     the assertion tagged by SYNTHESIS.
-  For example, \<^prop>\<open>\<^bold>p\<^bold>r\<^bold>o\<^bold>c f \<lbrace> X \<longmapsto> Y\<heavy_comma> SYNTHESIS Z \<rbrace>\<close> represents the procedure f generates
+  For example, \<^prop>\<open>\<^bold>p\<^bold>r\<^bold>o\<^bold>c f \<lbrace> X \<longmapsto> \<lambda>ret. Y\<heavy_comma> SYNTHESIS Z \<rbrace>\<close> represents the procedure f generates
     something that meets Z.
 
   During the reasoning, if a SYNTHESIS tags occurs in an antecedent, particularly in the post \<phi>-type,
-    like \<^prop>\<open>\<^bold>p\<^bold>r\<^bold>o\<^bold>c f \<lbrace> X \<longmapsto> Y\<heavy_comma> SYNTHESIS Z \<rbrace> \<Longrightarrow> C\<close>, it represents the reasoner needs to find
+    like \<^prop>\<open>\<^bold>p\<^bold>r\<^bold>o\<^bold>c f \<lbrace> X \<longmapsto> \<lambda>ret. Y\<heavy_comma> SYNTHESIS Z \<rbrace> \<Longrightarrow> C\<close>, it represents the reasoner needs to find
     some f that generates something meeting Z.
 
   Therefore, reasoning rules having the conclusion tagged by SYNTHESIS (in its post-type),
-    like \<^prop>\<open>A \<Longrightarrow> \<^bold>p\<^bold>r\<^bold>o\<^bold>c f \<lbrace> X \<longmapsto> Y\<heavy_comma> SYNTHESIS Z \<rbrace>\<close>, tell procedure f can generate what meets Z.
+    like \<^prop>\<open>A \<Longrightarrow> \<^bold>p\<^bold>r\<^bold>o\<^bold>c f \<lbrace> X \<longmapsto> \<lambda>ret. Y\<heavy_comma> SYNTHESIS Z \<rbrace>\<close>, tell procedure f can generate what meets Z.
 \<close>
-
-translations "SYNTHESIS (x \<Ztypecolon> T)" \<rightleftharpoons> "SYNTHESIS ELE (x \<Ztypecolon> T)"
 
 
 
 subsubsection \<open>Parse the Term to be Synthesised\<close>
 
-definition (in std) Synthesis_Parse :: \<open>'a \<Rightarrow> ('VAL,'FIC_N,'FIC) assn \<Rightarrow> bool\<close>
+definition (in std) Synthesis_Parse :: \<open>'a \<Rightarrow> ('ret \<Rightarrow> ('FIC_N,'FIC) assn) \<Rightarrow> bool\<close>
   where \<open>Synthesis_Parse input parsed \<longleftrightarrow> True\<close>
 
 text (in std) \<open>The system synthesises a program whose output meets the assertion given by user.
@@ -913,23 +907,20 @@ text (in std) \<open>The system synthesises a program whose output meets the ass
 
 context std begin
 
-lemma [\<phi>reason 9999 on \<open>Synthesis_Parse (?X'::('VAL,'FIC_N,'FIC)assn) ?X\<close>]:
+lemma [\<phi>reason 9999 on \<open>Synthesis_Parse (?X'::?'ret \<Rightarrow> ('FIC_N,'FIC)assn) ?X\<close>]:
   \<open>Synthesis_Parse X X\<close>
   unfolding Synthesis_Parse_def ..
 
-lemma [\<phi>reason 2000 on \<open>Synthesis_Parse (?X::'VAL set) ?Y\<close>]:
-  \<open>Synthesis_Parse X (VAL X)\<close>
-  unfolding Synthesis_Parse_def ..
-
-lemma [\<phi>reason 2000 on \<open>Synthesis_Parse (?X::('FIC_N \<Rightarrow> 'FIC) set) ?Y\<close>]:
-  \<open>Synthesis_Parse X (OBJ X)\<close>
+lemma [\<phi>reason 9999 on \<open>Synthesis_Parse (?X'::('FIC_N,'FIC)assn) ?X\<close>]:
+  \<open>Synthesis_Parse X (\<lambda>_. X)\<close>
   unfolding Synthesis_Parse_def ..
 
 lemma [\<phi>reason 30 
     on \<open>Synthesis_Parse ?x ?Y\<close>
     if no \<open>Synthesis_Parse (?x \<Ztypecolon> ?T) ?Y\<close>
-          \<open>Synthesis_Parse (?x::('VAL,'FIC_N,'FIC) assn) ?Y\<close>]:
-  \<open>Synthesis_Parse x (VAL x \<Ztypecolon> X)\<close>
+          \<open>Synthesis_Parse (?x::('FIC_N,'FIC) assn) ?Y\<close>
+          \<open>Synthesis_Parse (?x::?'ret \<Rightarrow> ('FIC_N,'FIC) assn) ?Y\<close>]:
+  \<open>Synthesis_Parse x (\<lambda>ret. x \<Ztypecolon> X ret)\<close>
   unfolding Synthesis_Parse_def ..
 
 end
@@ -952,10 +943,10 @@ lemma (in std) "__\<phi>synthesis__":
   " \<^bold>c\<^bold>u\<^bold>r\<^bold>r\<^bold>e\<^bold>n\<^bold>t blk [H] \<^bold>r\<^bold>e\<^bold>s\<^bold>u\<^bold>l\<^bold>t\<^bold>s \<^bold>i\<^bold>n S1
 \<Longrightarrow> SUBGOAL TOP_GOAL G
 \<Longrightarrow> Synthesis_Parse X X'
-\<Longrightarrow> \<^bold>p\<^bold>r\<^bold>o\<^bold>c f \<lbrace> S1 \<longmapsto> S2\<heavy_comma> SYNTHESIS X' \<^bold>t\<^bold>h\<^bold>r\<^bold>o\<^bold>w\<^bold>s E \<rbrace> \<^bold>@\<^bold>G\<^bold>O\<^bold>A\<^bold>L G
+\<Longrightarrow> \<^bold>p\<^bold>r\<^bold>o\<^bold>c f \<lbrace> S1 \<longmapsto> \<lambda>v. S2\<heavy_comma> SYNTHESIS X' v \<^bold>t\<^bold>h\<^bold>r\<^bold>o\<^bold>w\<^bold>s E \<rbrace> \<^bold>@\<^bold>G\<^bold>O\<^bold>A\<^bold>L G
 \<Longrightarrow> \<r>Success
 \<Longrightarrow> \<^bold>o\<^bold>b\<^bold>l\<^bold>i\<^bold>g\<^bold>a\<^bold>t\<^bold>i\<^bold>o\<^bold>n True
-\<Longrightarrow> \<^bold>p\<^bold>e\<^bold>n\<^bold>d\<^bold>i\<^bold>n\<^bold>g f \<^bold>o\<^bold>n blk [H] \<^bold>r\<^bold>e\<^bold>s\<^bold>u\<^bold>l\<^bold>t\<^bold>s \<^bold>i\<^bold>n S2\<heavy_comma> X' \<^bold>t\<^bold>h\<^bold>r\<^bold>o\<^bold>w\<^bold>s E"
+\<Longrightarrow> \<^bold>p\<^bold>e\<^bold>n\<^bold>d\<^bold>i\<^bold>n\<^bold>g f \<^bold>o\<^bold>n blk [H] \<^bold>r\<^bold>e\<^bold>s\<^bold>u\<^bold>l\<^bold>t\<^bold>s \<^bold>i\<^bold>n (\<lambda>v. S2\<heavy_comma> X' v) \<^bold>t\<^bold>h\<^bold>r\<^bold>o\<^bold>w\<^bold>s E"
   unfolding Synthesis_def GOAL_CTXT_def
   using \<phi>apply_proc .
 
@@ -975,14 +966,14 @@ subparagraph \<open>Rules to solve an antecedent by synthesis\<close>
 
 lemma (in std) [\<phi>reason 1400]:
   \<open> Synthesis_Parse X X'
-\<Longrightarrow> \<^bold>p\<^bold>r\<^bold>o\<^bold>c f \<lbrace> R1 \<longmapsto> R2\<heavy_comma> SYNTHESIS X' \<^bold>t\<^bold>h\<^bold>r\<^bold>o\<^bold>w\<^bold>s E \<rbrace> \<^bold>@\<^bold>G\<^bold>O\<^bold>A\<^bold>L G
-\<Longrightarrow> Synthesis_by X (\<^bold>p\<^bold>r\<^bold>o\<^bold>c f \<lbrace> R1 \<longmapsto> R2\<heavy_comma> SYNTHESIS X' \<^bold>t\<^bold>h\<^bold>r\<^bold>o\<^bold>w\<^bold>s E \<rbrace>) \<^bold>@\<^bold>G\<^bold>O\<^bold>A\<^bold>L G\<close>
+\<Longrightarrow> \<^bold>p\<^bold>r\<^bold>o\<^bold>c f \<lbrace> R1 \<longmapsto> \<lambda>ret. R2\<heavy_comma> SYNTHESIS X' ret \<^bold>t\<^bold>h\<^bold>r\<^bold>o\<^bold>w\<^bold>s E \<rbrace> \<^bold>@\<^bold>G\<^bold>O\<^bold>A\<^bold>L G
+\<Longrightarrow> Synthesis_by X (\<^bold>p\<^bold>r\<^bold>o\<^bold>c f \<lbrace> R1 \<longmapsto> \<lambda>ret. R2\<heavy_comma> SYNTHESIS X' ret \<^bold>t\<^bold>h\<^bold>r\<^bold>o\<^bold>w\<^bold>s E \<rbrace>) \<^bold>@\<^bold>G\<^bold>O\<^bold>A\<^bold>L G\<close>
   unfolding Synthesis_by_def .
 
 lemma (in std) [\<phi>reason 1200]:
   \<open> Synthesis_Parse X X'
-\<Longrightarrow> \<^bold>p\<^bold>r\<^bold>o\<^bold>c f \<lbrace> R1 \<longmapsto> R2\<heavy_comma> SYNTHESIS X' \<^bold>t\<^bold>h\<^bold>r\<^bold>o\<^bold>w\<^bold>s E \<rbrace> \<^bold>@\<^bold>G\<^bold>O\<^bold>A\<^bold>L G
-\<Longrightarrow> Synthesis_by X (\<^bold>p\<^bold>r\<^bold>o\<^bold>c f \<lbrace> R1 \<longmapsto> R2\<heavy_comma> X' \<^bold>t\<^bold>h\<^bold>r\<^bold>o\<^bold>w\<^bold>s E \<rbrace>) \<^bold>@\<^bold>G\<^bold>O\<^bold>A\<^bold>L G\<close>
+\<Longrightarrow> \<^bold>p\<^bold>r\<^bold>o\<^bold>c f \<lbrace> R1 \<longmapsto> \<lambda>ret. R2\<heavy_comma> SYNTHESIS X' ret \<^bold>t\<^bold>h\<^bold>r\<^bold>o\<^bold>w\<^bold>s E \<rbrace> \<^bold>@\<^bold>G\<^bold>O\<^bold>A\<^bold>L G
+\<Longrightarrow> Synthesis_by X (\<^bold>p\<^bold>r\<^bold>o\<^bold>c f \<lbrace> R1 \<longmapsto> \<lambda>ret. R2\<heavy_comma> X' ret \<^bold>t\<^bold>h\<^bold>r\<^bold>o\<^bold>w\<^bold>s E \<rbrace>) \<^bold>@\<^bold>G\<^bold>O\<^bold>A\<^bold>L G\<close>
   unfolding Synthesis_by_def Synthesis_def .
 
 lemma (in std) [\<phi>reason 1200]:
@@ -999,8 +990,8 @@ lemma (in std) [\<phi>reason 1200]:
 subsubsection \<open>General Synthesis Rules\<close>
 
 lemma (in std) [\<phi>reason 1200]:
-  \<open> \<^bold>p\<^bold>r\<^bold>o\<^bold>c F \<lbrace> R1 \<longmapsto> R2\<heavy_comma> SYNTHESIS VAL f x \<Ztypecolon> T \<rbrace>  \<^bold>@\<^bold>G\<^bold>O\<^bold>A\<^bold>L P
-\<Longrightarrow> \<^bold>p\<^bold>r\<^bold>o\<^bold>c F \<lbrace> R1 \<longmapsto> R2\<heavy_comma> SYNTHESIS VAL (case_named f (tag x)) \<Ztypecolon> T \<rbrace>  \<^bold>@\<^bold>G\<^bold>O\<^bold>A\<^bold>L P\<close>
+  \<open> \<^bold>p\<^bold>r\<^bold>o\<^bold>c F \<lbrace> R1 \<longmapsto> \<lambda>ret. R2\<heavy_comma> SYNTHESIS f x \<Ztypecolon> T ret \<rbrace>  \<^bold>@\<^bold>G\<^bold>O\<^bold>A\<^bold>L P
+\<Longrightarrow> \<^bold>p\<^bold>r\<^bold>o\<^bold>c F \<lbrace> R1 \<longmapsto> \<lambda>ret. R2\<heavy_comma> SYNTHESIS (case_named f (tag x)) \<Ztypecolon> T ret \<rbrace>  \<^bold>@\<^bold>G\<^bold>O\<^bold>A\<^bold>L P\<close>
   by simp
 
 
@@ -1178,7 +1169,21 @@ context std begin
 
 subparagraph \<open>Subtyping methods\<close>
 
-lemma \<phi>apply_subtyping_fast[\<phi>reason 2000 on \<open>
+lemma [\<phi>reason 3000 on \<open>
+  PROP \<phi>Application_Method (Trueprop (\<^bold>s\<^bold>u\<^bold>b\<^bold>t\<^bold>y\<^bold>p\<^bold>e ?x \<Ztypecolon> ?X \<longmapsto> ?T \<^bold>w\<^bold>i\<^bold>t\<^bold>h ?P))
+          (Trueprop (\<^bold>c\<^bold>u\<^bold>r\<^bold>r\<^bold>e\<^bold>n\<^bold>t ?blk [?RR] \<^bold>r\<^bold>e\<^bold>s\<^bold>u\<^bold>l\<^bold>t\<^bold>s \<^bold>i\<^bold>n ?x' \<Ztypecolon> ?X')) ?Result
+\<close>]:
+  \<open> PROP \<phi>Application_Method (Trueprop (\<^bold>s\<^bold>u\<^bold>b\<^bold>t\<^bold>y\<^bold>p\<^bold>e x \<Ztypecolon> X \<longmapsto> T \<^bold>w\<^bold>i\<^bold>t\<^bold>h P))
+      (Trueprop (\<^bold>c\<^bold>u\<^bold>r\<^bold>r\<^bold>e\<^bold>n\<^bold>t blk [R] \<^bold>r\<^bold>e\<^bold>s\<^bold>u\<^bold>l\<^bold>t\<^bold>s \<^bold>i\<^bold>n Void\<heavy_comma> x' \<Ztypecolon> X'))
+      (Trueprop ((\<^bold>c\<^bold>u\<^bold>r\<^bold>r\<^bold>e\<^bold>n\<^bold>t blk [R] \<^bold>r\<^bold>e\<^bold>s\<^bold>u\<^bold>l\<^bold>t\<^bold>s \<^bold>i\<^bold>n T') \<and> P'))
+\<Longrightarrow> PROP \<phi>Application_Method (Trueprop (\<^bold>s\<^bold>u\<^bold>b\<^bold>t\<^bold>y\<^bold>p\<^bold>e x \<Ztypecolon> X \<longmapsto> T \<^bold>w\<^bold>i\<^bold>t\<^bold>h P))
+      (Trueprop (\<^bold>c\<^bold>u\<^bold>r\<^bold>r\<^bold>e\<^bold>n\<^bold>t blk [R] \<^bold>r\<^bold>e\<^bold>s\<^bold>u\<^bold>l\<^bold>t\<^bold>s \<^bold>i\<^bold>n x' \<Ztypecolon> X'))
+      (Trueprop ((\<^bold>c\<^bold>u\<^bold>r\<^bold>r\<^bold>e\<^bold>n\<^bold>t blk [R] \<^bold>r\<^bold>e\<^bold>s\<^bold>u\<^bold>l\<^bold>t\<^bold>s \<^bold>i\<^bold>n T') \<and> P'))\<close>
+  by simp
+
+
+
+lemma \<phi>apply_subtyping_fast[\<phi>reason 1800 on \<open>
   PROP \<phi>Application_Method (Trueprop (\<^bold>s\<^bold>u\<^bold>b\<^bold>t\<^bold>y\<^bold>p\<^bold>e ?S \<longmapsto> ?T \<^bold>w\<^bold>i\<^bold>t\<^bold>h ?P))
           (Trueprop (\<^bold>c\<^bold>u\<^bold>r\<^bold>r\<^bold>e\<^bold>n\<^bold>t ?blk [?RR] \<^bold>r\<^bold>e\<^bold>s\<^bold>u\<^bold>l\<^bold>t\<^bold>s \<^bold>i\<^bold>n ?S)) ?Result
 \<close>]:
@@ -1189,12 +1194,22 @@ lemma \<phi>apply_subtyping_fast[\<phi>reason 2000 on \<open>
   unfolding \<phi>Application_Method_def \<phi>Application_def
   using "\<phi>cast_P" .
 
+lemma [\<phi>reason 1500 on \<open>
+  PROP \<phi>Application_Method (Trueprop (\<^bold>s\<^bold>u\<^bold>b\<^bold>t\<^bold>y\<^bold>p\<^bold>e ?S \<longmapsto> ?T \<^bold>w\<^bold>i\<^bold>t\<^bold>h ?P))
+          (Trueprop (\<^bold>c\<^bold>u\<^bold>r\<^bold>r\<^bold>e\<^bold>n\<^bold>t ?blk [?RR] \<^bold>r\<^bold>e\<^bold>s\<^bold>u\<^bold>l\<^bold>t\<^bold>s \<^bold>i\<^bold>n ?R\<heavy_comma> ?S)) ?Result
+\<close>]:
+  \<open> PROP \<phi>Application_Success
+\<Longrightarrow> PROP \<phi>Application_Method (Trueprop (\<^bold>s\<^bold>u\<^bold>b\<^bold>t\<^bold>y\<^bold>p\<^bold>e S \<longmapsto> T \<^bold>w\<^bold>i\<^bold>t\<^bold>h P))
+      (Trueprop (\<^bold>c\<^bold>u\<^bold>r\<^bold>r\<^bold>e\<^bold>n\<^bold>t blk [RR] \<^bold>r\<^bold>e\<^bold>s\<^bold>u\<^bold>l\<^bold>t\<^bold>s \<^bold>i\<^bold>n R\<heavy_comma> S))
+      (Trueprop ((\<^bold>c\<^bold>u\<^bold>r\<^bold>r\<^bold>e\<^bold>n\<^bold>t blk [RR] \<^bold>r\<^bold>e\<^bold>s\<^bold>u\<^bold>l\<^bold>t\<^bold>s \<^bold>i\<^bold>n R\<heavy_comma> T) \<and> P))\<close>
+  unfolding \<phi>Application_Method_def \<phi>Application_def
+  using "\<phi>cast_P" \<phi>cast_intro_frame by blast
 
 lemma \<phi>apply_subtyping_fully[\<phi>reason on \<open>
   PROP \<phi>Application_Method (Trueprop (\<^bold>s\<^bold>u\<^bold>b\<^bold>t\<^bold>y\<^bold>p\<^bold>e ?S' \<longmapsto> ?T' \<^bold>w\<^bold>i\<^bold>t\<^bold>h ?P))
       (Trueprop (\<^bold>c\<^bold>u\<^bold>r\<^bold>r\<^bold>e\<^bold>n\<^bold>t ?blk [?RR] \<^bold>r\<^bold>e\<^bold>s\<^bold>u\<^bold>l\<^bold>t\<^bold>s \<^bold>i\<^bold>n ?S)) ?Result
 \<close>]:
-  "IntroFrameVar R S'' S' T T' E E'
+  "IntroFrameVar R S'' S' T T'
 \<Longrightarrow> SUBGOAL TOP_GOAL G
 \<Longrightarrow> \<^bold>s\<^bold>u\<^bold>b\<^bold>t\<^bold>y\<^bold>p\<^bold>e S \<longmapsto> \<blangle> S'' \<brangle> \<^bold>w\<^bold>i\<^bold>t\<^bold>h Any  \<^bold>@\<^bold>G\<^bold>O\<^bold>A\<^bold>L G
 \<Longrightarrow> SOLVE_SUBGOAL G
@@ -1209,6 +1224,7 @@ lemma \<phi>apply_subtyping_fully[\<phi>reason on \<open>
   by (metis (no_types, lifting))
 
 
+(*
 lemma [\<phi>reason 2000 on \<open>
   PROP \<phi>Application_Method (Trueprop (\<^bold>s\<^bold>u\<^bold>b\<^bold>t\<^bold>y\<^bold>p\<^bold>e ?S \<longmapsto> ?T \<^bold>w\<^bold>i\<^bold>t\<^bold>h ?P))
           (Trueprop (\<^bold>c\<^bold>u\<^bold>r\<^bold>r\<^bold>e\<^bold>n\<^bold>t ?blk [?RR] \<^bold>r\<^bold>e\<^bold>s\<^bold>u\<^bold>l\<^bold>t\<^bold>s \<^bold>i\<^bold>n VAL ?S)) ?Result
@@ -1261,7 +1277,7 @@ lemma [\<phi>reason 2000 on \<open>
       (Trueprop ((\<^bold>c\<^bold>u\<^bold>r\<^bold>r\<^bold>e\<^bold>n\<^bold>t blk [RR] \<^bold>r\<^bold>e\<^bold>s\<^bold>u\<^bold>l\<^bold>t\<^bold>s \<^bold>i\<^bold>n R\<heavy_comma> VAL T) \<and> P))\<close>
   unfolding \<phi>Application_Method_def \<phi>Application_def
   using "\<phi>cast_P" cast_val_\<phi>app[unfolded Argument_def] \<phi>cast_intro_frame by metis
-
+*)
 
 subparagraph \<open>Procedure methods\<close>
 
@@ -1281,7 +1297,7 @@ lemma \<phi>apply_proc_fully[\<phi>reason on
     \<open>PROP \<phi>Application_Method (Trueprop (\<^bold>p\<^bold>r\<^bold>o\<^bold>c ?f \<lbrace> ?S' \<longmapsto> ?T' \<^bold>t\<^bold>h\<^bold>r\<^bold>o\<^bold>w\<^bold>s ?E \<rbrace>))
             (Trueprop (\<^bold>c\<^bold>u\<^bold>r\<^bold>r\<^bold>e\<^bold>n\<^bold>t ?blk [?RR] \<^bold>r\<^bold>e\<^bold>s\<^bold>u\<^bold>l\<^bold>t\<^bold>s \<^bold>i\<^bold>n ?S)) ?Result\<close>
 ]:
-  \<open> IntroFrameVar R S'' S' T T' E'' E'
+  \<open> IntroFrameVar' R S'' S' T T' E'' E'
 \<Longrightarrow> SUBGOAL TOP_GOAL G
 \<Longrightarrow> \<^bold>s\<^bold>u\<^bold>b\<^bold>t\<^bold>y\<^bold>p\<^bold>e S \<longmapsto> \<blangle> S'' \<brangle> \<^bold>w\<^bold>i\<^bold>t\<^bold>h P  \<^bold>@\<^bold>G\<^bold>O\<^bold>A\<^bold>L G
 \<Longrightarrow> SOLVE_SUBGOAL G
@@ -1291,9 +1307,10 @@ lemma \<phi>apply_proc_fully[\<phi>reason on
 \<Longrightarrow> PROP \<phi>Application_Method (Trueprop (\<^bold>p\<^bold>r\<^bold>o\<^bold>c f \<lbrace> S' \<longmapsto> T' \<^bold>t\<^bold>h\<^bold>r\<^bold>o\<^bold>w\<^bold>s E' \<rbrace>))
     (Trueprop (\<^bold>c\<^bold>u\<^bold>r\<^bold>r\<^bold>e\<^bold>n\<^bold>t blk [RR] \<^bold>r\<^bold>e\<^bold>s\<^bold>u\<^bold>l\<^bold>t\<^bold>s \<^bold>i\<^bold>n S))
     (Trueprop (\<^bold>p\<^bold>e\<^bold>n\<^bold>d\<^bold>i\<^bold>n\<^bold>g f \<^bold>o\<^bold>n blk [RR] \<^bold>r\<^bold>e\<^bold>s\<^bold>u\<^bold>l\<^bold>t\<^bold>s \<^bold>i\<^bold>n T \<^bold>t\<^bold>h\<^bold>r\<^bold>o\<^bold>w\<^bold>s E))\<close>
-  unfolding \<phi>Application_Method_def \<phi>Application_def IntroFrameVar_def
+  unfolding \<phi>Application_Method_def \<phi>Application_def IntroFrameVar'_def
     GOAL_CTXT_def FOCUS_TAG_def Simplify_def
-  using "\<phi>cast" \<phi>apply_proc \<phi>frame[where R=R] by meson
+  using "\<phi>cast" \<phi>apply_proc \<phi>frame[where R=R]
+  by (metis \<phi>CONSEQ' \<phi>frame cast_id)
 
 end
 
@@ -1302,7 +1319,20 @@ paragraph \<open>Applying on a Block / End a Block\<close>
 
 definition \<open>Exhaustive_Abstract f f' \<longleftrightarrow> (f = f')\<close>
 
-lemma Exhaustive_Abstract_I: \<open>Exhaustive_Abstract f f\<close> unfolding Exhaustive_Abstract_def ..
+consts procedure_equivalent :: mode
+named_theorems procedure_equivalent_simps
+
+declare proc_bind_SKIP[folded Return_def, procedure_equivalent_simps]
+  proc_bind_SKIP[procedure_equivalent_simps]
+  proc_bind_assoc[procedure_equivalent_simps]
+
+\<phi>reasoner procedure_equivalent 1200 (conclusion \<open>Premise procedure_equivalent ?P\<close>)
+  = (rule Premise_I; simp only: procedure_equivalent_simps; fail)
+
+lemma Exhaustive_Abstract_I:
+  \<open> Premise procedure_equivalent (f = f')
+\<Longrightarrow> Exhaustive_Abstract f f'\<close>
+  unfolding Exhaustive_Abstract_def Premise_def by simp
 
 \<phi>reasoner_ML Exhaustive_Abstract 1200 (conclusion \<open>Exhaustive_Abstract ?f ?f'\<close>) = \<open>
 let
@@ -1345,13 +1375,15 @@ in
 end
 \<close>
 
-lemma (in std) [\<phi>reason 1200]:
+lemma (in std) [\<phi>reason 1200 on \<open>
+  PROP \<phi>Application_Conv (Trueprop (\<^bold>p\<^bold>r\<^bold>o\<^bold>c ?f \<lbrace> ?X \<longmapsto> ?Y \<^bold>t\<^bold>h\<^bold>r\<^bold>o\<^bold>w\<^bold>s ?E \<rbrace>)) (Trueprop (\<^bold>p\<^bold>r\<^bold>o\<^bold>c ?f' \<lbrace> ?X' \<longmapsto> ?Y' \<^bold>t\<^bold>h\<^bold>r\<^bold>o\<^bold>w\<^bold>s ?E' \<rbrace>))
+\<close>]:
   \<open> Exhaustive_Abstract f f'
 \<Longrightarrow> SUBGOAL TOP_GOAL G1
 \<Longrightarrow> \<^bold>s\<^bold>u\<^bold>b\<^bold>t\<^bold>y\<^bold>p\<^bold>e X' \<longmapsto> \<blangle> X \<brangle> \<^bold>w\<^bold>i\<^bold>t\<^bold>h Any1  \<^bold>@\<^bold>G\<^bold>O\<^bold>A\<^bold>L G1
 \<Longrightarrow> SOLVE_SUBGOAL G1
 \<Longrightarrow> SUBGOAL TOP_GOAL G2
-\<Longrightarrow> \<^bold>s\<^bold>u\<^bold>b\<^bold>t\<^bold>y\<^bold>p\<^bold>e Y  \<longmapsto> \<blangle> Y' \<brangle> \<^bold>w\<^bold>i\<^bold>t\<^bold>h Any2  \<^bold>@\<^bold>G\<^bold>O\<^bold>A\<^bold>L G2
+\<Longrightarrow> (\<And>ret. \<^bold>s\<^bold>u\<^bold>b\<^bold>t\<^bold>y\<^bold>p\<^bold>e Y ret \<longmapsto> \<blangle> Y' ret \<brangle> \<^bold>w\<^bold>i\<^bold>t\<^bold>h Any2  \<^bold>@\<^bold>G\<^bold>O\<^bold>A\<^bold>L G2)
 \<Longrightarrow> SOLVE_SUBGOAL G2
 \<Longrightarrow> SUBGOAL TOP_GOAL G3
 \<Longrightarrow> \<^bold>s\<^bold>u\<^bold>b\<^bold>t\<^bold>y\<^bold>p\<^bold>e E  \<longmapsto> \<blangle> E' \<brangle> \<^bold>w\<^bold>i\<^bold>t\<^bold>h Any3  \<^bold>@\<^bold>G\<^bold>O\<^bold>A\<^bold>L G3
@@ -1367,7 +1399,7 @@ lemma (in std) [\<phi>reason 1200]:
 section \<open>Elementary \<phi>-Types\<close>
 
 
-subsubsection \<open>Type Level Subjection\<close>
+subsection \<open>Type Level Subjection\<close>
 
 definition SubjectionTY :: \<open>('a,'b) \<phi> \<Rightarrow> bool \<Rightarrow> ('a,'b) \<phi>\<close> (infixl "\<phi>\<^bold>s\<^bold>u\<^bold>b\<^bold>j" 25)
   where \<open> (T \<phi>\<^bold>s\<^bold>u\<^bold>b\<^bold>j P) = (\<lambda>x. x \<Ztypecolon> T \<^bold>s\<^bold>u\<^bold>b\<^bold>j P) \<close>
@@ -1381,7 +1413,7 @@ lemma SubjectionTY_inhabited[\<phi>reason_elim!, elim!]:
   unfolding SubjectionTY_expn using Subjection_inhabited .
 
 
-subsubsection \<open>Type Level Existential Quantification\<close>
+subsection \<open>Type Level Existential Quantification\<close>
 
 definition ExTyp :: \<open>('c \<Rightarrow> ('a, 'b) \<phi>) \<Rightarrow> ('a, 'c \<Rightarrow> 'b)\<phi>\<close> (binder "\<exists>\<phi>" 10)
   where \<open>ExTyp T = (\<lambda>x. (\<exists>*c. x c \<Ztypecolon> T c))\<close>
@@ -1433,7 +1465,7 @@ lemma ExTyp_inhabited[elim!, \<phi>reason_elim!]:
 
 
 
-subsubsection \<open>Prod\<close>
+subsection \<open>Prod\<close>
 
 definition \<phi>Prod :: " ('concrete::times, 'abs_a) \<phi> \<Rightarrow> ('concrete, 'abs_b) \<phi> \<Rightarrow> ('concrete, 'abs_a \<times> 'abs_b) \<phi>" (infixr "\<^emph>" 70)
   where "A \<^emph> B = (\<lambda>(a,b). A a * B b)"
@@ -1449,8 +1481,8 @@ lemma \<phi>Prod_inhabited[elim!,\<phi>reason_elim!]:
 lemma \<phi>Prod_split: "((a,b) \<Ztypecolon> A \<^emph> B) = (a \<Ztypecolon> A) * (b \<Ztypecolon> B)"
   by (simp add: \<phi>expns set_eq_iff)
 
-lemma (in std) SepNu_to_SepSet: "(OBJ (a,b) \<Ztypecolon> A \<^emph> B) = (OBJ a \<Ztypecolon> A) * (OBJ b \<Ztypecolon> B)"
-  by (simp add: \<phi>expns set_eq_iff times_list_def)
+(*lemma (in std) SepNu_to_SepSet: "(OBJ (a,b) \<Ztypecolon> A \<^emph> B) = (OBJ a \<Ztypecolon> A) * (OBJ b \<Ztypecolon> B)"
+  by (simp add: \<phi>expns set_eq_iff times_list_def) *)
 
 lemma [\<phi>reason on \<open>\<^bold>s\<^bold>u\<^bold>b\<^bold>t\<^bold>y\<^bold>p\<^bold>e (?x,?y) \<Ztypecolon> ?N \<^emph> ?M \<longmapsto> (?x',?y') \<Ztypecolon> ?N' \<^emph> ?M' \<^bold>w\<^bold>i\<^bold>t\<^bold>h ?P\<close>]:
   "\<^bold>s\<^bold>u\<^bold>b\<^bold>t\<^bold>y\<^bold>p\<^bold>e x \<Ztypecolon> N \<longmapsto> x' \<Ztypecolon> N' \<^bold>w\<^bold>i\<^bold>t\<^bold>h P1 \<Longrightarrow> \<^bold>s\<^bold>u\<^bold>b\<^bold>t\<^bold>y\<^bold>p\<^bold>e y \<Ztypecolon> M \<longmapsto> y' \<Ztypecolon> M' \<^bold>w\<^bold>i\<^bold>t\<^bold>h P2 \<Longrightarrow>
@@ -1475,7 +1507,7 @@ lemma heap_split_by_addr_set: "P (h |` (MemAddress ` S)) (h |` (- (MemAddress ` 
 
 
 
-subsubsection \<open>Identity\<close>
+subsection \<open>Identity\<close>
 
 definition Identity :: " ('a,'a) \<phi> " where "Identity x = {x}"
 
@@ -1499,7 +1531,7 @@ lemma from_Identity_\<phi>app:
   unfolding Subty_def Premise_def by (simp add: \<phi>expns)
 
 
-subsubsection \<open>Stepwise Abstraction\<close>
+subsection \<open>Stepwise Abstraction\<close>
 
 definition \<phi>Composition :: \<open>('v,'a) \<phi> \<Rightarrow> ('a,'b) \<phi> \<Rightarrow> ('v,'b) \<phi>\<close> (infixl "\<Zcomp>" 75)
   where \<open>\<phi>Composition T U = (\<lambda>x. (y \<Ztypecolon> T \<^bold>s\<^bold>u\<^bold>b\<^bold>j y. y \<in> U x))\<close>
@@ -1514,7 +1546,7 @@ lemma \<phi>Composition_inhabited[elim,\<phi>reason_elim!]:
 
 
 
-subsubsection \<open>Refinement\<close>
+subsection \<open>Refinement\<close>
 
 definition NuRefine :: " ('a, 'b) \<phi> \<Rightarrow> 'b set \<Rightarrow> ('a, 'b) \<phi> " (infixl "<where>" 80)
   where "(N <where> T) x = {p. (x \<in> T \<and>p \<in> (x \<Ztypecolon> N))}"
@@ -1541,7 +1573,7 @@ lemma refine_\<phi>app:
   unfolding Subty_def by (simp add: \<phi>expns)
 
 
-subsubsection \<open>Forward Simulation\<close>
+subsection \<open>Forward Simulation\<close>
 
 definition F_simulate :: \<open>('VAL,'a) \<phi> \<Rightarrow> ('VAL,'b) \<phi> \<Rightarrow> ('VAL \<Rightarrow> 'VAL, 'a \<Rightarrow> 'b) \<phi>\<close> (infixr "\<Rrightarrow>" 25)
     \<comment> \<open>Forward Simulation\<close>
@@ -1557,7 +1589,7 @@ lemma F_simulate_inhabited[\<phi>expns]:
 
 
 
-subsubsection \<open>Down Lifting\<close> (*depreciated*)
+subsection \<open>Down Lifting\<close> (*depreciated*)
 
 definition DownLift :: "('a, 'b) \<phi> \<Rightarrow> ('c \<Rightarrow> 'b) \<Rightarrow> ('a,'c) \<phi>" (infixl "<down-lift>" 80)
   where "DownLift N g x = (g x \<Ztypecolon> N)"
@@ -1584,7 +1616,7 @@ lemma "\<down>lift_\<phi>app": "\<^bold>p\<^bold>a\<^bold>r\<^bold>a\<^bold>m g 
 
 
 
-subsubsection \<open>Up Lifting\<close> (*depreciated*)
+subsection \<open>Up Lifting\<close> (*depreciated*)
 
 definition UpLift :: "('a, 'c) \<phi> \<Rightarrow> ('c \<Rightarrow> 'b) \<Rightarrow> ('a,'b) \<phi>" (infixl "<up-lift>" 80)
   where "UpLift N f x = {p. (\<exists>y. f y = x \<and> p \<in> (y \<Ztypecolon> N))}"
@@ -1628,7 +1660,89 @@ lemma "\<^bold>s\<^bold>u\<^bold>b\<^bold>t\<^bold>y\<^bold>p\<^bold>e x \<Ztype
 (* lemma "\<phi>Equal (N <up-lift> f) can_eq eq \<longleftrightarrow> \<phi>Equal N (inv_imagep can_eq f) (inv_imagep eq f)"
   unfolding \<phi>Equal_def by (auto 0 6) *)
 
-subsubsection \<open>Representative Type Tagging\<close>
+
+subsection \<open>Value\<close>
+
+definition (in std) Val :: \<open>'VAL \<Rightarrow> ('VAL, 'a) \<phi> \<Rightarrow> ('FIC_N \<Rightarrow> 'FIC, 'a) \<phi>\<close>
+  where \<open>Val val T = (\<lambda>x. Void \<^bold>s\<^bold>u\<^bold>b\<^bold>j val \<in> (x \<Ztypecolon> T))\<close>
+
+lemma (in std) Val_expn [\<phi>expns]:
+  \<open>(x \<Ztypecolon> Val val T) = (Void \<^bold>s\<^bold>u\<^bold>b\<^bold>j val \<in> (x \<Ztypecolon> T))\<close>
+  unfolding Val_def \<phi>Type_def by (simp add: \<phi>expns)
+
+lemma (in std) Val_inhabited [\<phi>reason_elim, elim!]:
+  \<open>Inhabited (x \<Ztypecolon> Val val T) \<Longrightarrow> (Inhabited (x \<Ztypecolon> T) \<Longrightarrow> C) \<Longrightarrow> C\<close>
+  unfolding Inhabited_def by (simp add: \<phi>expns) blast
+
+lemma (in std) Val_cast [\<phi>reason]:
+  \<open> \<^bold>s\<^bold>u\<^bold>b\<^bold>t\<^bold>y\<^bold>p\<^bold>e y \<Ztypecolon> U \<longmapsto> x \<Ztypecolon> T \<^bold>w\<^bold>i\<^bold>t\<^bold>h P
+\<Longrightarrow> \<^bold>s\<^bold>u\<^bold>b\<^bold>t\<^bold>y\<^bold>p\<^bold>e y \<Ztypecolon> Val v U \<longmapsto> x \<Ztypecolon> Val v T \<^bold>w\<^bold>i\<^bold>t\<^bold>h P\<close>
+  unfolding Subty_def by (simp add: \<phi>expns)
+
+subsubsection \<open>Syntax\<close>
+
+context std begin
+ML  \<open>@{term \<open>\<^bold>p\<^bold>r\<^bold>o\<^bold>c f \<lbrace> X \<longmapsto> Y \<rbrace>\<close>}\<close>
+end
+
+consts val_syntax :: "unit \<Rightarrow> unit" ("\<^bold>v\<^bold>a\<^bold>l _" [22] 21) (*the type is senseless because
+  it will and should be translated during type-checking phase.
+  Any occurrence not translated means the misusing.*)
+ML_file \<open>library/procedure_syntax.ML\<close>
+
+
+subsubsection \<open>Simplification Rules\<close>
+
+lemma (in std) [\<phi>programming_simps]:
+    \<open>Val raw (ExTyp T) = (\<exists>\<phi> c. Val raw (T c))\<close>
+  by (rule \<phi>Type_eqI) (simp add: \<phi>expns)
+
+lemma (in std) [\<phi>programming_simps]:
+    \<open>Val raw (T \<phi>\<^bold>s\<^bold>u\<^bold>b\<^bold>j P) = (Val raw T \<phi>\<^bold>s\<^bold>u\<^bold>b\<^bold>j P)\<close>
+  by (rule \<phi>Type_eqI) (simp add: \<phi>expns)
+
+
+subsubsection \<open>Application Methods for Subtyping\<close>
+
+lemma (in std) [\<phi>reason 2000 on \<open>
+  PROP \<phi>Application_Method (Trueprop (\<^bold>s\<^bold>u\<^bold>b\<^bold>t\<^bold>y\<^bold>p\<^bold>e ?x \<Ztypecolon> ?T \<longmapsto> ?y \<Ztypecolon> ?U \<^bold>w\<^bold>i\<^bold>t\<^bold>h ?P))
+          (Trueprop (\<^bold>c\<^bold>u\<^bold>r\<^bold>r\<^bold>e\<^bold>n\<^bold>t ?blk [?RR] \<^bold>r\<^bold>e\<^bold>s\<^bold>u\<^bold>l\<^bold>t\<^bold>s \<^bold>i\<^bold>n ?R\<heavy_comma> ?x \<Ztypecolon> Val ?raw ?T)) ?Result
+\<close> if no \<open>
+  PROP \<phi>Application_Method (Trueprop (\<^bold>s\<^bold>u\<^bold>b\<^bold>t\<^bold>y\<^bold>p\<^bold>e ?x \<Ztypecolon> Val ?raw ?T \<longmapsto> ?y \<Ztypecolon> ?U \<^bold>w\<^bold>i\<^bold>t\<^bold>h ?P))
+          (Trueprop (\<^bold>c\<^bold>u\<^bold>r\<^bold>r\<^bold>e\<^bold>n\<^bold>t ?blk [?RR] \<^bold>r\<^bold>e\<^bold>s\<^bold>u\<^bold>l\<^bold>t\<^bold>s \<^bold>i\<^bold>n ?R)) ?Result
+\<close>]:
+  \<open> PROP \<phi>Application_Success
+\<Longrightarrow> PROP \<phi>Application_Method (Trueprop (\<^bold>s\<^bold>u\<^bold>b\<^bold>t\<^bold>y\<^bold>p\<^bold>e x \<Ztypecolon> T \<longmapsto> y \<Ztypecolon> U \<^bold>w\<^bold>i\<^bold>t\<^bold>h P))
+      (Trueprop (\<^bold>c\<^bold>u\<^bold>r\<^bold>r\<^bold>e\<^bold>n\<^bold>t blk [RR] \<^bold>r\<^bold>e\<^bold>s\<^bold>u\<^bold>l\<^bold>t\<^bold>s \<^bold>i\<^bold>n R\<heavy_comma> x \<Ztypecolon> Val raw T))
+      (Trueprop ((\<^bold>c\<^bold>u\<^bold>r\<^bold>r\<^bold>e\<^bold>n\<^bold>t blk [RR] \<^bold>r\<^bold>e\<^bold>s\<^bold>u\<^bold>l\<^bold>t\<^bold>s \<^bold>i\<^bold>n R\<heavy_comma> y \<Ztypecolon> Val raw U) \<and> P))\<close>
+  unfolding \<phi>Application_Method_def \<phi>Application_def
+  using "\<phi>cast_P" Val_cast \<phi>cast_intro_frame by metis
+
+
+lemma (in std) [\<phi>reason 2000 on \<open>
+  PROP \<phi>Application_Method (Trueprop (\<^bold>s\<^bold>u\<^bold>b\<^bold>t\<^bold>y\<^bold>p\<^bold>e ?x' \<Ztypecolon> ?T' \<longmapsto> ?y \<Ztypecolon> ?U \<^bold>w\<^bold>i\<^bold>t\<^bold>h ?P))
+      (Trueprop (\<^bold>c\<^bold>u\<^bold>r\<^bold>r\<^bold>e\<^bold>n\<^bold>t ?blk [?RR] \<^bold>r\<^bold>e\<^bold>s\<^bold>u\<^bold>l\<^bold>t\<^bold>s \<^bold>i\<^bold>n ?R\<heavy_comma> ?x \<Ztypecolon> Val ?raw ?T)) ?Result
+\<close> if no \<open>
+  PROP \<phi>Application_Method (Trueprop (\<^bold>s\<^bold>u\<^bold>b\<^bold>t\<^bold>y\<^bold>p\<^bold>e ?x \<Ztypecolon> Val ?raw ?T \<longmapsto> ?y \<Ztypecolon> ?U \<^bold>w\<^bold>i\<^bold>t\<^bold>h ?P))
+          (Trueprop (\<^bold>c\<^bold>u\<^bold>r\<^bold>r\<^bold>e\<^bold>n\<^bold>t ?blk [?RR] \<^bold>r\<^bold>e\<^bold>s\<^bold>u\<^bold>l\<^bold>t\<^bold>s \<^bold>i\<^bold>n ?R)) ?Result
+\<close>]:
+  \<open> SUBGOAL TOP_GOAL G
+\<Longrightarrow> \<^bold>s\<^bold>u\<^bold>b\<^bold>t\<^bold>y\<^bold>p\<^bold>e x \<Ztypecolon> T \<longmapsto> x' \<Ztypecolon> T' \<^bold>w\<^bold>i\<^bold>t\<^bold>h Any
+\<Longrightarrow> SOLVE_SUBGOAL G
+\<Longrightarrow> PROP \<phi>Application_Success
+\<Longrightarrow> \<^bold>o\<^bold>b\<^bold>l\<^bold>i\<^bold>g\<^bold>a\<^bold>t\<^bold>i\<^bold>o\<^bold>n True
+\<Longrightarrow> PROP \<phi>Application_Method (Trueprop (\<^bold>s\<^bold>u\<^bold>b\<^bold>t\<^bold>y\<^bold>p\<^bold>e x' \<Ztypecolon> T' \<longmapsto> y \<Ztypecolon> U \<^bold>w\<^bold>i\<^bold>t\<^bold>h P))
+      (Trueprop (\<^bold>c\<^bold>u\<^bold>r\<^bold>r\<^bold>e\<^bold>n\<^bold>t blk [RR] \<^bold>r\<^bold>e\<^bold>s\<^bold>u\<^bold>l\<^bold>t\<^bold>s \<^bold>i\<^bold>n R\<heavy_comma> x \<Ztypecolon> Val raw T))
+      (Trueprop ((\<^bold>c\<^bold>u\<^bold>r\<^bold>r\<^bold>e\<^bold>n\<^bold>t blk [RR] \<^bold>r\<^bold>e\<^bold>s\<^bold>u\<^bold>l\<^bold>t\<^bold>s \<^bold>i\<^bold>n R\<heavy_comma> y \<Ztypecolon> Val raw U) \<and> P))\<close>
+  unfolding \<phi>Application_Method_def \<phi>Application_def
+  using "\<phi>cast_P" Val_cast \<phi>cast_intro_frame by metis
+
+
+
+
+
+
+subsection \<open>Representative Type Tagging\<close>
 
 definition (in std) Of_Type :: \<open>('VAL,'a) \<phi> \<Rightarrow> 'TY \<Rightarrow> ('VAL,'a) \<phi>\<close> (infix "<of-type>" 23)
   where \<open>(T <of-type> TY) = (\<lambda>x. x \<Ztypecolon> T \<^bold>s\<^bold>u\<^bold>b\<^bold>j \<phi>SemType (x \<Ztypecolon> T) TY)\<close>
@@ -1648,7 +1762,9 @@ lemma (in std) [\<phi>reason]:
 \<Longrightarrow> \<^bold>s\<^bold>u\<^bold>b\<^bold>t\<^bold>y\<^bold>p\<^bold>e x \<Ztypecolon> T \<longmapsto> y \<Ztypecolon> U <of-type> TY \<^bold>w\<^bold>i\<^bold>t\<^bold>h P\<close>
   unfolding Subty_def by (simp add: \<phi>expns)
 
-subsubsection \<open>Misc.\<close>
+
+
+subsection \<open>Misc.\<close>
 
 definition Function_over :: \<open>('a,'b) \<phi> \<Rightarrow> 'c \<Rightarrow> ('a, 'c \<Rightarrow> 'b) \<phi>\<close> (infix "<func-over>" 40)
   where \<open>(T <func-over> x) = (\<lambda>f. f x \<Ztypecolon> T)\<close>
@@ -1687,16 +1803,16 @@ lemma [\<phi>reason 2000]:
 \<Longrightarrow> \<^bold>s\<^bold>u\<^bold>b\<^bold>t\<^bold>y\<^bold>p\<^bold>e f \<Ztypecolon> T <func-over> x \<longmapsto> Y \<^bold>w\<^bold>i\<^bold>t\<^bold>h P\<close>
   unfolding Subty_def by (simp add: \<phi>expns)
 
-lemma (in std) [\<phi>reason 1200 on \<open>Synthesis_Parse ?input (VAL ?f \<Ztypecolon> ?T <func-over> ?x)\<close>]:
-  \<open> Synthesis_Parse input (VAL fx \<Ztypecolon> T)
+lemma (in std) [\<phi>reason 1200 on \<open>Synthesis_Parse ?input (\<lambda>v. ?f \<Ztypecolon> ?T v <func-over> ?x)\<close>]:
+  \<open> Synthesis_Parse input (\<lambda>v. fx \<Ztypecolon> T v)
 \<Longrightarrow> lambda_abstraction x fx f
-\<Longrightarrow> Synthesis_Parse input (VAL f \<Ztypecolon> T <func-over> x)\<close>
+\<Longrightarrow> Synthesis_Parse input (\<lambda>v. f \<Ztypecolon> T v <func-over> x)\<close>
   unfolding Synthesis_Parse_def ..
 
 
 lemma (in std) [\<phi>reason 1200]:
-  \<open> \<^bold>p\<^bold>r\<^bold>o\<^bold>c g \<lbrace> R1 \<longmapsto> R2\<heavy_comma> SYNTHESIS VAL f x \<Ztypecolon> T \<rbrace>  \<^bold>@\<^bold>G\<^bold>O\<^bold>A\<^bold>L P
-\<Longrightarrow> \<^bold>p\<^bold>r\<^bold>o\<^bold>c g \<lbrace> R1 \<longmapsto> R2\<heavy_comma> SYNTHESIS VAL f \<Ztypecolon> T <func-over> x \<rbrace>  \<^bold>@\<^bold>G\<^bold>O\<^bold>A\<^bold>L P\<close>
+  \<open> \<^bold>p\<^bold>r\<^bold>o\<^bold>c g \<lbrace> R1 \<longmapsto> \<lambda>v. R2\<heavy_comma> SYNTHESIS f x \<Ztypecolon> T v \<rbrace>  \<^bold>@\<^bold>G\<^bold>O\<^bold>A\<^bold>L P
+\<Longrightarrow> \<^bold>p\<^bold>r\<^bold>o\<^bold>c g \<lbrace> R1 \<longmapsto> \<lambda>v. R2\<heavy_comma> SYNTHESIS f \<Ztypecolon> T v <func-over> x \<rbrace>  \<^bold>@\<^bold>G\<^bold>O\<^bold>A\<^bold>L P\<close>
   unfolding Synthesis_def lambda_abstraction_def by (simp add: \<phi>expns)
 
 
@@ -1768,19 +1884,19 @@ lemma (in std) "_\<phi>cast_internal_rule_":
 \<Longrightarrow> \<^bold>o\<^bold>b\<^bold>l\<^bold>i\<^bold>g\<^bold>a\<^bold>t\<^bold>i\<^bold>o\<^bold>n True
 \<Longrightarrow> \<^bold>c\<^bold>u\<^bold>r\<^bold>r\<^bold>e\<^bold>n\<^bold>t blk [H] \<^bold>r\<^bold>e\<^bold>s\<^bold>u\<^bold>l\<^bold>t\<^bold>s \<^bold>i\<^bold>n T'"
   unfolding CurrentConstruction_def GOAL_CTXT_def Subty_def FOCUS_TAG_def
-  by (cases blk, simp_all add: pair_All \<phi>expns) blast
+  by (simp_all add: pair_All \<phi>expns) blast
 
 lemma (in std) "_\<phi>cast_internal_rule_'":
   " \<^bold>p\<^bold>e\<^bold>n\<^bold>d\<^bold>i\<^bold>n\<^bold>g f \<^bold>o\<^bold>n blk [H] \<^bold>r\<^bold>e\<^bold>s\<^bold>u\<^bold>l\<^bold>t\<^bold>s \<^bold>i\<^bold>n T \<^bold>t\<^bold>h\<^bold>r\<^bold>o\<^bold>w\<^bold>s E
-\<Longrightarrow> \<^bold>s\<^bold>u\<^bold>b\<^bold>t\<^bold>y\<^bold>p\<^bold>e T \<longmapsto> \<blangle> T' \<brangle> \<^bold>w\<^bold>i\<^bold>t\<^bold>h Any  \<^bold>@\<^bold>G\<^bold>O\<^bold>A\<^bold>L TOP_GOAL
+\<Longrightarrow> (\<And>v. \<^bold>s\<^bold>u\<^bold>b\<^bold>t\<^bold>y\<^bold>p\<^bold>e T v \<longmapsto> \<blangle> T' v \<brangle> \<^bold>w\<^bold>i\<^bold>t\<^bold>h Any  \<^bold>@\<^bold>G\<^bold>O\<^bold>A\<^bold>L TOP_GOAL)
 \<Longrightarrow> \<r>Success
 \<Longrightarrow> \<^bold>o\<^bold>b\<^bold>l\<^bold>i\<^bold>g\<^bold>a\<^bold>t\<^bold>i\<^bold>o\<^bold>n True
 \<Longrightarrow> \<^bold>p\<^bold>e\<^bold>n\<^bold>d\<^bold>i\<^bold>n\<^bold>g f \<^bold>o\<^bold>n blk [H] \<^bold>r\<^bold>e\<^bold>s\<^bold>u\<^bold>l\<^bold>t\<^bold>s \<^bold>i\<^bold>n T' \<^bold>t\<^bold>h\<^bold>r\<^bold>o\<^bold>w\<^bold>s E"
   unfolding FOCUS_TAG_def Subty_def PendingConstruction_def bind_def GOAL_CTXT_def
-  by (cases blk, auto simp add: \<phi>expns LooseStateTy_expn') blast+
+  by (auto simp add: \<phi>expns LooseStateTy_expn') blast+
 
 
-subsubsection \<open>General Rules\<close>
+(* subsubsection \<open>General Rules\<close>
 
 lemma (in std) [\<phi>reason 2000 on \<open>\<^bold>s\<^bold>u\<^bold>b\<^bold>t\<^bold>y\<^bold>p\<^bold>e VAL ?X \<longmapsto> VAL ?Y \<^bold>w\<^bold>i\<^bold>t\<^bold>h ?P\<close>]:
   \<open> \<^bold>s\<^bold>u\<^bold>b\<^bold>t\<^bold>y\<^bold>p\<^bold>e X \<longmapsto> Y \<^bold>w\<^bold>i\<^bold>t\<^bold>h P
@@ -1790,7 +1906,7 @@ lemma (in std) [\<phi>reason 2000 on \<open>\<^bold>s\<^bold>u\<^bold>b\<^bold>t
 lemma (in std) [\<phi>reason 2000 on \<open>\<^bold>s\<^bold>u\<^bold>b\<^bold>t\<^bold>y\<^bold>p\<^bold>e OBJ ?X \<longmapsto> OBJ ?Y \<^bold>w\<^bold>i\<^bold>t\<^bold>h ?P\<close>]:
   \<open> \<^bold>s\<^bold>u\<^bold>b\<^bold>t\<^bold>y\<^bold>p\<^bold>e X \<longmapsto> Y \<^bold>w\<^bold>i\<^bold>t\<^bold>h P
 \<Longrightarrow> \<^bold>s\<^bold>u\<^bold>b\<^bold>t\<^bold>y\<^bold>p\<^bold>e OBJ X \<longmapsto> OBJ Y \<^bold>w\<^bold>i\<^bold>t\<^bold>h P\<close>
-  unfolding Subty_def by (simp add: \<phi>expns, blast)
+  unfolding Subty_def by (simp add: \<phi>expns, blast) *)
 
 
 subsubsection \<open>Case Analysis\<close>
@@ -1985,6 +2101,14 @@ lemma [\<phi>reason 2500 on \<open>\<^bold>s\<^bold>u\<^bold>b\<^bold>t\<^bold>y
 \<Longrightarrow> \<^bold>s\<^bold>u\<^bold>b\<^bold>t\<^bold>y\<^bold>p\<^bold>e A + B \<longmapsto> X \<^bold>w\<^bold>i\<^bold>t\<^bold>h P1 \<or> P2 \<^bold>@\<^bold>G\<^bold>O\<^bold>A\<^bold>L G\<close>
   unfolding cast_def plus_set_def by simp
 
+lemma [\<phi>reason 2500 on \<open>\<^bold>s\<^bold>u\<^bold>b\<^bold>t\<^bold>y\<^bold>p\<^bold>e ?R\<heavy_comma> (?A + ?B) \<longmapsto> ?X \<^bold>w\<^bold>i\<^bold>t\<^bold>h ?P \<^bold>@\<^bold>G\<^bold>O\<^bold>A\<^bold>L ?G\<close>]:
+  \<open> SUBGOAL G G1
+\<Longrightarrow> \<^bold>s\<^bold>u\<^bold>b\<^bold>t\<^bold>y\<^bold>p\<^bold>e R\<heavy_comma> B \<longmapsto> X \<^bold>w\<^bold>i\<^bold>t\<^bold>h P1 \<^bold>@\<^bold>G\<^bold>O\<^bold>A\<^bold>L G1
+\<Longrightarrow> SOLVE_SUBGOAL G1
+\<Longrightarrow> \<^bold>s\<^bold>u\<^bold>b\<^bold>t\<^bold>y\<^bold>p\<^bold>e R\<heavy_comma> A \<longmapsto> X \<^bold>w\<^bold>i\<^bold>t\<^bold>h P2 \<^bold>@\<^bold>G\<^bold>O\<^bold>A\<^bold>L G
+\<Longrightarrow> \<^bold>s\<^bold>u\<^bold>b\<^bold>t\<^bold>y\<^bold>p\<^bold>e R\<heavy_comma> A + B \<longmapsto> X \<^bold>w\<^bold>i\<^bold>t\<^bold>h P1 \<or> P2 \<^bold>@\<^bold>G\<^bold>O\<^bold>A\<^bold>L G\<close>
+  unfolding cast_def by (simp add: distrib_left)
+
 lemma [\<phi>reason 800]:
   \<open> SUBGOAL G G1
 \<Longrightarrow> \<^bold>s\<^bold>u\<^bold>b\<^bold>t\<^bold>y\<^bold>p\<^bold>e X \<longmapsto> \<blangle> A \<brangle> \<^bold>w\<^bold>i\<^bold>t\<^bold>h P \<^bold>@\<^bold>G\<^bold>O\<^bold>A\<^bold>L G1
@@ -1998,6 +2122,20 @@ lemma [\<phi>reason 800]:
 \<Longrightarrow> SOLVE_SUBGOAL G1
 \<Longrightarrow> \<^bold>s\<^bold>u\<^bold>b\<^bold>t\<^bold>y\<^bold>p\<^bold>e X \<longmapsto> \<blangle> A + B \<brangle> \<^bold>w\<^bold>i\<^bold>t\<^bold>h P \<^bold>@\<^bold>G\<^bold>O\<^bold>A\<^bold>L G\<close>
   unfolding cast_def plus_set_def by simp
+
+lemma [\<phi>reason 800]:
+  \<open> SUBGOAL G G1
+\<Longrightarrow> \<^bold>s\<^bold>u\<^bold>b\<^bold>t\<^bold>y\<^bold>p\<^bold>e X \<longmapsto> R\<heavy_comma> \<blangle> A \<brangle> \<^bold>w\<^bold>i\<^bold>t\<^bold>h P \<^bold>@\<^bold>G\<^bold>O\<^bold>A\<^bold>L G1
+\<Longrightarrow> SOLVE_SUBGOAL G1
+\<Longrightarrow> \<^bold>s\<^bold>u\<^bold>b\<^bold>t\<^bold>y\<^bold>p\<^bold>e X \<longmapsto> R\<heavy_comma> \<blangle> A + B \<brangle> \<^bold>w\<^bold>i\<^bold>t\<^bold>h P \<^bold>@\<^bold>G\<^bold>O\<^bold>A\<^bold>L G\<close>
+  unfolding cast_def by (simp add: distrib_left) 
+
+lemma [\<phi>reason 800]:
+  \<open> SUBGOAL G G1
+\<Longrightarrow> \<^bold>s\<^bold>u\<^bold>b\<^bold>t\<^bold>y\<^bold>p\<^bold>e X \<longmapsto> R\<heavy_comma> \<blangle> B \<brangle> \<^bold>w\<^bold>i\<^bold>t\<^bold>h P \<^bold>@\<^bold>G\<^bold>O\<^bold>A\<^bold>L G1
+\<Longrightarrow> SOLVE_SUBGOAL G1
+\<Longrightarrow> \<^bold>s\<^bold>u\<^bold>b\<^bold>t\<^bold>y\<^bold>p\<^bold>e X \<longmapsto> R\<heavy_comma> \<blangle> A + B \<brangle> \<^bold>w\<^bold>i\<^bold>t\<^bold>h P \<^bold>@\<^bold>G\<^bold>O\<^bold>A\<^bold>L G\<close>
+  unfolding cast_def by (simp add: distrib_left)
 
 subsubsection \<open>General\<close>
 
@@ -2025,54 +2163,54 @@ lemma [\<phi>reason 2500 on \<open>\<^bold>s\<^bold>u\<^bold>b\<^bold>t\<^bold>y
   unfolding cast_def pair_forall
   by (simp add: \<phi>expns times_list_def)
 
-lemma [\<phi>reason on \<open>\<^bold>s\<^bold>u\<^bold>b\<^bold>t\<^bold>y\<^bold>p\<^bold>e ?R \<heavy_comma> (OBJ ?H) \<longmapsto> ?R' \<heavy_comma> \<blangle> ?X \<brangle> \<^bold>w\<^bold>i\<^bold>t\<^bold>h ?P \<^bold>@\<^bold>G\<^bold>O\<^bold>A\<^bold>L ?G\<close>
-    if no \<open>\<^bold>s\<^bold>u\<^bold>b\<^bold>t\<^bold>y\<^bold>p\<^bold>e ?R \<heavy_comma> (OBJ ?H) \<longmapsto> ?R' \<heavy_comma> \<blangle> OBJ ?X \<brangle> \<^bold>w\<^bold>i\<^bold>t\<^bold>h ?P \<^bold>@\<^bold>G\<^bold>O\<^bold>A\<^bold>L ?G\<close>]:
-  " \<^bold>s\<^bold>u\<^bold>b\<^bold>t\<^bold>y\<^bold>p\<^bold>e R \<longmapsto> R' \<heavy_comma> \<blangle> X \<brangle> \<^bold>w\<^bold>i\<^bold>t\<^bold>h P \<^bold>@\<^bold>G\<^bold>O\<^bold>A\<^bold>L G
-\<Longrightarrow> \<^bold>s\<^bold>u\<^bold>b\<^bold>t\<^bold>y\<^bold>p\<^bold>e R \<heavy_comma> (OBJ H) \<longmapsto> R' \<heavy_comma> (OBJ H) \<heavy_comma> \<blangle> X \<brangle> \<^bold>w\<^bold>i\<^bold>t\<^bold>h P \<^bold>@\<^bold>G\<^bold>O\<^bold>A\<^bold>L G "
-  unfolding cast_def pair_forall
-  by (smt (z3) OBJ_comm mult.assoc old.prod.exhaust set_mult_expn)
-
 
 subsubsection \<open>Value\<close>
 
-lemma [\<phi>reason 2000 on \<open>\<^bold>s\<^bold>u\<^bold>b\<^bold>t\<^bold>y\<^bold>p\<^bold>e ?R \<heavy_comma> (VAL ?V) \<longmapsto> ?R''' \<heavy_comma> \<blangle> VAL ?X \<brangle> \<^bold>w\<^bold>i\<^bold>t\<^bold>h ?P \<^bold>@\<^bold>G\<^bold>O\<^bold>A\<^bold>L ?G\<close>]:
-  " \<^bold>s\<^bold>u\<^bold>b\<^bold>t\<^bold>y\<^bold>p\<^bold>e V \<longmapsto> X \<^bold>w\<^bold>i\<^bold>t\<^bold>h P
-\<Longrightarrow> \<^bold>s\<^bold>u\<^bold>b\<^bold>t\<^bold>y\<^bold>p\<^bold>e R \<heavy_comma> (VAL V) \<longmapsto> R \<heavy_comma> \<blangle> VAL X \<brangle> \<^bold>w\<^bold>i\<^bold>t\<^bold>h P \<^bold>@\<^bold>G\<^bold>O\<^bold>A\<^bold>L G"
+text \<open>The rules require the same values are alpha-conversible. \<close>
+
+lemma [\<phi>reason 2000 on \<open>\<^bold>s\<^bold>u\<^bold>b\<^bold>t\<^bold>y\<^bold>p\<^bold>e ?R\<heavy_comma> ?y \<Ztypecolon> Val ?v ?U \<longmapsto> ?R''' \<heavy_comma> \<blangle> ?x \<Ztypecolon> Val ?v ?T \<brangle> \<^bold>w\<^bold>i\<^bold>t\<^bold>h ?P \<^bold>@\<^bold>G\<^bold>O\<^bold>A\<^bold>L ?G\<close>]:
+  " \<^bold>s\<^bold>u\<^bold>b\<^bold>t\<^bold>y\<^bold>p\<^bold>e y \<Ztypecolon> U \<longmapsto> x \<Ztypecolon> T \<^bold>w\<^bold>i\<^bold>t\<^bold>h P
+\<Longrightarrow> \<^bold>s\<^bold>u\<^bold>b\<^bold>t\<^bold>y\<^bold>p\<^bold>e R \<heavy_comma> y \<Ztypecolon> Val v U \<longmapsto> R \<heavy_comma> \<blangle> x \<Ztypecolon> Val v T \<brangle> \<^bold>w\<^bold>i\<^bold>t\<^bold>h P \<^bold>@\<^bold>G\<^bold>O\<^bold>A\<^bold>L G"
   unfolding cast_def pair_forall
   by (simp add: \<phi>expns times_list_def) metis
 
+lemma [\<phi>reason 1800 on \<open>\<^bold>s\<^bold>u\<^bold>b\<^bold>t\<^bold>y\<^bold>p\<^bold>e ?R\<heavy_comma> ?X \<longmapsto> ?R'''\<heavy_comma> \<blangle> ?x \<Ztypecolon> Val ?v ?T \<brangle> \<^bold>w\<^bold>i\<^bold>t\<^bold>h ?P \<^bold>@\<^bold>G\<^bold>O\<^bold>A\<^bold>L ?G\<close>]:
+  " \<^bold>s\<^bold>u\<^bold>b\<^bold>t\<^bold>y\<^bold>p\<^bold>e R \<longmapsto> R'\<heavy_comma> \<blangle> x \<Ztypecolon> Val v T \<brangle> \<^bold>w\<^bold>i\<^bold>t\<^bold>h P \<^bold>@\<^bold>G\<^bold>O\<^bold>A\<^bold>L G
+\<Longrightarrow> \<^bold>s\<^bold>u\<^bold>b\<^bold>t\<^bold>y\<^bold>p\<^bold>e R \<heavy_comma> X \<longmapsto> R'\<heavy_comma> X\<heavy_comma> \<blangle> x \<Ztypecolon> Val v T \<brangle> \<^bold>w\<^bold>i\<^bold>t\<^bold>h P \<^bold>@\<^bold>G\<^bold>O\<^bold>A\<^bold>L G"
+  unfolding cast_def pair_forall
+  by (simp add: \<phi>expns times_list_def) blast
 
-subsubsection \<open>Object\<close>
+subsubsection \<open>General Search\<close>
 
-lemma [\<phi>reason 100 on \<open>\<^bold>s\<^bold>u\<^bold>b\<^bold>t\<^bold>y\<^bold>p\<^bold>e ?R \<heavy_comma> OBJ ?H \<longmapsto> ?R''' * \<blangle> OBJ ?X \<brangle> \<^bold>w\<^bold>i\<^bold>t\<^bold>h ?P \<^bold>@\<^bold>G\<^bold>O\<^bold>A\<^bold>L ?G\<close>]: \<comment> \<open>attempts the immediate cell\<close>
+lemma [\<phi>reason 100 on \<open>\<^bold>s\<^bold>u\<^bold>b\<^bold>t\<^bold>y\<^bold>p\<^bold>e ?R \<heavy_comma> ?H \<longmapsto> ?R''' * \<blangle> ?X \<brangle> \<^bold>w\<^bold>i\<^bold>t\<^bold>h ?P \<^bold>@\<^bold>G\<^bold>O\<^bold>A\<^bold>L ?G\<close>]: \<comment> \<open>attempts the immediate cell\<close>
   " CHK_SUBGOAL G
-  \<Longrightarrow> \<^bold>s\<^bold>u\<^bold>b\<^bold>t\<^bold>y\<^bold>p\<^bold>e OBJ H \<longmapsto> H'\<heavy_comma> OBJ X \<^bold>w\<^bold>i\<^bold>t\<^bold>h P
-  \<Longrightarrow> \<^bold>s\<^bold>u\<^bold>b\<^bold>t\<^bold>y\<^bold>p\<^bold>e R\<heavy_comma> OBJ H \<longmapsto> R\<heavy_comma> H'\<heavy_comma> \<blangle> OBJ X \<brangle> \<^bold>w\<^bold>i\<^bold>t\<^bold>h P \<^bold>@\<^bold>G\<^bold>O\<^bold>A\<^bold>L G"
+  \<Longrightarrow> \<^bold>s\<^bold>u\<^bold>b\<^bold>t\<^bold>y\<^bold>p\<^bold>e H \<longmapsto> H'\<heavy_comma> X \<^bold>w\<^bold>i\<^bold>t\<^bold>h P
+  \<Longrightarrow> \<^bold>s\<^bold>u\<^bold>b\<^bold>t\<^bold>y\<^bold>p\<^bold>e R\<heavy_comma> H \<longmapsto> R\<heavy_comma> H'\<heavy_comma> \<blangle> X \<brangle> \<^bold>w\<^bold>i\<^bold>t\<^bold>h P \<^bold>@\<^bold>G\<^bold>O\<^bold>A\<^bold>L G"
   unfolding cast_def
   by (simp add: \<phi>expns times_list_def del: split_paired_All split_paired_Ex)  (metis mult.assoc)
 
 
-lemma [\<phi>reason 70 on \<open>\<^bold>s\<^bold>u\<^bold>b\<^bold>t\<^bold>y\<^bold>p\<^bold>e ?R \<heavy_comma> OBJ ?H \<longmapsto> ?R''' \<heavy_comma> \<blangle> OBJ ?X \<brangle> \<^bold>w\<^bold>i\<^bold>t\<^bold>h ?P \<^bold>@\<^bold>G\<^bold>O\<^bold>A\<^bold>L ?G\<close>]: \<comment> \<open>or attempts the next cell, if still not succeeded\<close>
+lemma [\<phi>reason 70 on \<open>\<^bold>s\<^bold>u\<^bold>b\<^bold>t\<^bold>y\<^bold>p\<^bold>e ?R \<heavy_comma> ?H \<longmapsto> ?R''' \<heavy_comma> \<blangle> ?X \<brangle> \<^bold>w\<^bold>i\<^bold>t\<^bold>h ?P \<^bold>@\<^bold>G\<^bold>O\<^bold>A\<^bold>L ?G\<close>]: \<comment> \<open>or attempts the next cell, if still not succeeded\<close>
   " CHK_SUBGOAL G
-  \<Longrightarrow> \<^bold>s\<^bold>u\<^bold>b\<^bold>t\<^bold>y\<^bold>p\<^bold>e R \<longmapsto> R' \<heavy_comma> \<blangle> OBJ X \<brangle> \<^bold>w\<^bold>i\<^bold>t\<^bold>h P \<^bold>@\<^bold>G\<^bold>O\<^bold>A\<^bold>L G
-  \<Longrightarrow> \<^bold>s\<^bold>u\<^bold>b\<^bold>t\<^bold>y\<^bold>p\<^bold>e R \<heavy_comma> OBJ H \<longmapsto> R' \<heavy_comma> OBJ H \<heavy_comma> \<blangle> OBJ X \<brangle> \<^bold>w\<^bold>i\<^bold>t\<^bold>h P \<^bold>@\<^bold>G\<^bold>O\<^bold>A\<^bold>L G "
+  \<Longrightarrow> \<^bold>s\<^bold>u\<^bold>b\<^bold>t\<^bold>y\<^bold>p\<^bold>e R \<longmapsto> R' \<heavy_comma> \<blangle> X \<brangle> \<^bold>w\<^bold>i\<^bold>t\<^bold>h P \<^bold>@\<^bold>G\<^bold>O\<^bold>A\<^bold>L G
+  \<Longrightarrow> \<^bold>s\<^bold>u\<^bold>b\<^bold>t\<^bold>y\<^bold>p\<^bold>e R \<heavy_comma> H \<longmapsto> R' \<heavy_comma> H \<heavy_comma> \<blangle> X \<brangle> \<^bold>w\<^bold>i\<^bold>t\<^bold>h P \<^bold>@\<^bold>G\<^bold>O\<^bold>A\<^bold>L G "
   unfolding cast_def pair_forall
   by (simp add: \<phi>expns times_list_def) (metis fun_mult_norm mult.commute)
 
-lemma [\<phi>reason 10 on \<open>\<^bold>s\<^bold>u\<^bold>b\<^bold>t\<^bold>y\<^bold>p\<^bold>e OBJ ?a \<Zinj> ?x \<Ztypecolon> ?T \<longmapsto> ?R''' \<heavy_comma> OBJ ?a' \<Zinj> ?x' \<Ztypecolon> ?T' \<^bold>w\<^bold>i\<^bold>t\<^bold>h ?P\<close>]:
+lemma [\<phi>reason 10 on \<open>\<^bold>s\<^bold>u\<^bold>b\<^bold>t\<^bold>y\<^bold>p\<^bold>e ?a \<Zinj> ?x \<Ztypecolon> ?T \<longmapsto> ?R''' \<heavy_comma> ?a' \<Zinj> ?x' \<Ztypecolon> ?T' \<^bold>w\<^bold>i\<^bold>t\<^bold>h ?P\<close>]:
   "\<^bold>s\<^bold>i\<^bold>m\<^bold>p\<^bold>r\<^bold>e\<^bold>m a = a' \<Longrightarrow>
    \<^bold>s\<^bold>u\<^bold>b\<^bold>t\<^bold>y\<^bold>p\<^bold>e a \<Zinj> x \<Ztypecolon> T \<longmapsto> a' \<Zinj> x' \<Ztypecolon> T' \<^bold>w\<^bold>i\<^bold>t\<^bold>h P \<Longrightarrow>
-   \<^bold>s\<^bold>u\<^bold>b\<^bold>t\<^bold>y\<^bold>p\<^bold>e OBJ a \<Zinj> x \<Ztypecolon> T \<longmapsto> 1 \<heavy_comma> OBJ a' \<Zinj> x' \<Ztypecolon> T' \<^bold>w\<^bold>i\<^bold>t\<^bold>h P"
-  unfolding cast_def pair_forall by (simp add: \<phi>expns) blast
+   \<^bold>s\<^bold>u\<^bold>b\<^bold>t\<^bold>y\<^bold>p\<^bold>e a \<Zinj> x \<Ztypecolon> T \<longmapsto> 1 \<heavy_comma> a' \<Zinj> x' \<Ztypecolon> T' \<^bold>w\<^bold>i\<^bold>t\<^bold>h P"
+  unfolding cast_def pair_forall by (simp add: \<phi>expns)
 
-lemma [\<phi>reason 1200 on \<open>\<^bold>s\<^bold>u\<^bold>b\<^bold>t\<^bold>y\<^bold>p\<^bold>e ?R \<heavy_comma> ?V \<longmapsto> ?R''' \<heavy_comma> \<blangle> OBJ ?X \<brangle> \<^bold>w\<^bold>i\<^bold>t\<^bold>h ?P \<^bold>@\<^bold>G\<^bold>O\<^bold>A\<^bold>L ?G\<close>
-    if no \<open>\<^bold>s\<^bold>u\<^bold>b\<^bold>t\<^bold>y\<^bold>p\<^bold>e ?R \<heavy_comma> OBJ ?V \<longmapsto> ?R''' \<heavy_comma> \<blangle> OBJ ?X \<brangle> \<^bold>w\<^bold>i\<^bold>t\<^bold>h ?P \<^bold>@\<^bold>G\<^bold>O\<^bold>A\<^bold>L ?G\<close>
-          \<open>\<^bold>s\<^bold>u\<^bold>b\<^bold>t\<^bold>y\<^bold>p\<^bold>e ?R \<heavy_comma> Void \<longmapsto> ?R''' \<heavy_comma> \<blangle> OBJ ?X \<brangle> \<^bold>w\<^bold>i\<^bold>t\<^bold>h ?P \<^bold>@\<^bold>G\<^bold>O\<^bold>A\<^bold>L ?G\<close>
+lemma [\<phi>reason 1200 on \<open>\<^bold>s\<^bold>u\<^bold>b\<^bold>t\<^bold>y\<^bold>p\<^bold>e ?R \<heavy_comma> ?x \<Ztypecolon> Val ?v ?V \<longmapsto> ?R''' \<heavy_comma> \<blangle> ?X \<brangle> \<^bold>w\<^bold>i\<^bold>t\<^bold>h ?P \<^bold>@\<^bold>G\<^bold>O\<^bold>A\<^bold>L ?G\<close>
+    if no \<open>\<^bold>s\<^bold>u\<^bold>b\<^bold>t\<^bold>y\<^bold>p\<^bold>e ?R \<heavy_comma> Void \<longmapsto> ?R''' \<heavy_comma> \<blangle> ?X \<brangle> \<^bold>w\<^bold>i\<^bold>t\<^bold>h ?P \<^bold>@\<^bold>G\<^bold>O\<^bold>A\<^bold>L ?G\<close>
 ]:
-  " \<^bold>s\<^bold>u\<^bold>b\<^bold>t\<^bold>y\<^bold>p\<^bold>e R \<longmapsto> R' \<heavy_comma> \<blangle> OBJ X \<brangle> \<^bold>w\<^bold>i\<^bold>t\<^bold>h P \<^bold>@\<^bold>G\<^bold>O\<^bold>A\<^bold>L G
-  \<Longrightarrow> \<^bold>s\<^bold>u\<^bold>b\<^bold>t\<^bold>y\<^bold>p\<^bold>e R \<heavy_comma> V \<longmapsto> R' \<heavy_comma> V \<heavy_comma> \<blangle> OBJ X \<brangle> \<^bold>w\<^bold>i\<^bold>t\<^bold>h P \<^bold>@\<^bold>G\<^bold>O\<^bold>A\<^bold>L G"
+  " \<^bold>s\<^bold>u\<^bold>b\<^bold>t\<^bold>y\<^bold>p\<^bold>e R \<longmapsto> R' \<heavy_comma> \<blangle> X \<brangle> \<^bold>w\<^bold>i\<^bold>t\<^bold>h P \<^bold>@\<^bold>G\<^bold>O\<^bold>A\<^bold>L G
+  \<Longrightarrow> \<^bold>s\<^bold>u\<^bold>b\<^bold>t\<^bold>y\<^bold>p\<^bold>e R \<heavy_comma> x \<Ztypecolon> Val v V \<longmapsto> R' \<heavy_comma> x \<Ztypecolon> Val v V \<heavy_comma> \<blangle> X \<brangle> \<^bold>w\<^bold>i\<^bold>t\<^bold>h P \<^bold>@\<^bold>G\<^bold>O\<^bold>A\<^bold>L G"
   unfolding cast_def pair_forall
-  by (smt (z3) OBJ_comm mult.assoc old.prod.exhaust set_mult_expn)
+  by (smt (verit, best) mult.assoc mult.commute set_mult_expn)
+  
 
 
 (* lemma [\<phi>reason 1200
@@ -2787,74 +2925,61 @@ section \<open>Construction Elements\<close>
 
 context std_sem begin
 
-definition \<phi>M_assert :: \<open>bool \<Rightarrow> ('VAL,'RES_N,'RES) proc\<close>
-  where \<open>\<phi>M_assert P = (\<lambda>s. if P then Success s else Fail)\<close>
+definition \<phi>M_assert :: \<open>bool \<Rightarrow> (unit,'RES_N,'RES) proc\<close>
+  where \<open>\<phi>M_assert P = (\<lambda>s. if P then Success () s else Fail)\<close>
 
-definition \<phi>M_assume :: \<open>bool \<Rightarrow> ('VAL,'RES_N,'RES) proc\<close>
-  where \<open>\<phi>M_assume P = (\<lambda>s. if P then Success s else PartialCorrect)\<close>
+definition \<phi>M_assume :: \<open>bool \<Rightarrow> (unit,'RES_N,'RES) proc\<close>
+  where \<open>\<phi>M_assume P = (\<lambda>s. if P then Success () s else PartialCorrect)\<close>
 
-definition \<phi>M_get_Val :: \<open>('VAL \<Rightarrow> ('VAL,'RES_N,'RES) proc) \<Rightarrow> ('VAL,'RES_N,'RES) proc\<close>
-  where \<open>\<phi>M_get_Val F = (\<lambda>(vs,res). case vs of v#vs' \<Rightarrow> F v (vs',res) | _ \<Rightarrow> Fail)\<close>
-
-definition \<phi>M_put_Val :: \<open>'VAL \<Rightarrow> ('VAL,'RES_N,'RES) proc\<close>
-  where \<open>\<phi>M_put_Val V = (\<lambda>(vs,res). Success (V#vs,res))\<close>
-
-definition \<phi>M_getV :: \<open>'TY \<Rightarrow> ('VAL \<Rightarrow> 'a) \<Rightarrow> ('a \<Rightarrow> ('VAL,'RES_N,'RES) proc) \<Rightarrow> ('VAL,'RES_N,'RES) proc\<close>
-  where \<open>\<phi>M_getV TY VDT_dest F = \<phi>M_get_Val (\<lambda>v. \<phi>M_assert (v \<in> Well_Type TY) \<ggreater> F (VDT_dest v))\<close>
+definition \<phi>M_getV :: \<open>'TY \<Rightarrow> ('VAL \<Rightarrow> 'v) \<Rightarrow> 'VAL \<Rightarrow> ('v \<Rightarrow> ('y::value,'RES_N,'RES) proc) \<Rightarrow> ('y,'RES_N,'RES) proc\<close>
+  where \<open>\<phi>M_getV TY VDT_dest v F = (\<phi>M_assert (v \<in> Well_Type TY) \<ggreater> F (VDT_dest v))\<close>
 
 end
 
 context std begin
 
 declare \<phi>SEQ[\<phi>reason!]
-declare \<phi>SKIP[\<phi>reason! on \<open>\<^bold>p\<^bold>r\<^bold>o\<^bold>c SKIP \<lbrace> ?A \<longmapsto> ?B \<rbrace>\<close>]
 
 lemma \<phi>M_assert[\<phi>reason! on \<open>\<^bold>p\<^bold>r\<^bold>o\<^bold>c \<phi>M_assert ?P \<lbrace> ?A \<longmapsto> ?B \<rbrace>\<close>]:
-  \<open>(Inhabited X \<Longrightarrow> P) \<Longrightarrow> \<^bold>p\<^bold>r\<^bold>o\<^bold>c \<phi>M_assert P \<lbrace> X \<longmapsto> X \<rbrace>\<close>
+  \<open>(Inhabited X \<Longrightarrow> P) \<Longrightarrow> \<^bold>p\<^bold>r\<^bold>o\<^bold>c \<phi>M_assert P \<lbrace> X \<longmapsto> \<lambda>_. X \<rbrace>\<close>
   unfolding \<phi>Procedure_def \<phi>M_assert_def by (auto simp add: \<phi>expns Inhabited_def)
 
 lemma \<phi>M_assert_True[simp]:
-  \<open>\<phi>M_assert True = Success\<close>
+  \<open>\<phi>M_assert True = Success ()\<close>
   unfolding \<phi>M_assert_def by simp
 
 lemma \<phi>M_assert':
   \<open>P \<Longrightarrow> Q (F args) \<Longrightarrow> Q ((\<phi>M_assert P \<ggreater> F) args)\<close>
-  unfolding \<phi>M_assert_def instr_comp_def bind_def by simp
+  unfolding \<phi>M_assert_def bind_def by simp
 
-lemma \<phi>M_assume[\<phi>reason!]: \<open>(P \<Longrightarrow> \<^bold>p\<^bold>r\<^bold>o\<^bold>c F \<lbrace> X \<longmapsto> Y \<rbrace>) \<Longrightarrow> \<^bold>p\<^bold>r\<^bold>o\<^bold>c (\<phi>M_assume P \<ggreater> F) \<lbrace> X \<longmapsto> Y \<rbrace>\<close>
-  unfolding \<phi>Procedure_def \<phi>M_assume_def instr_comp_def bind_def by force
+lemma \<phi>M_assume[\<phi>reason!]:
+  \<open>(P \<Longrightarrow> \<^bold>p\<^bold>r\<^bold>o\<^bold>c F \<lbrace> X \<longmapsto> Y \<rbrace>) \<Longrightarrow> \<^bold>p\<^bold>r\<^bold>o\<^bold>c (\<phi>M_assume P \<ggreater> F) \<lbrace> X \<longmapsto> Y \<rbrace>\<close>
+  unfolding \<phi>Procedure_def \<phi>M_assume_def bind_def by force
 
 lemma throw_\<phi>app:
-  \<open>\<^bold>p\<^bold>r\<^bold>o\<^bold>c Exception \<lbrace> X \<longmapsto> 0 \<^bold>t\<^bold>h\<^bold>r\<^bold>o\<^bold>w\<^bold>s X \<rbrace>\<close>
+  \<open>\<^bold>p\<^bold>r\<^bold>o\<^bold>c Exception \<lbrace> X \<longmapsto> \<lambda>_. 0 \<^bold>t\<^bold>h\<^bold>r\<^bold>o\<^bold>w\<^bold>s X \<rbrace>\<close>
   unfolding \<phi>Procedure_def by simp
 
 lemma \<phi>M_tail_left:  \<open>\<^bold>p\<^bold>r\<^bold>o\<^bold>c F \<lbrace> 1\<heavy_comma> X \<longmapsto> Y \<rbrace> \<Longrightarrow> \<^bold>p\<^bold>r\<^bold>o\<^bold>c F \<lbrace> X \<longmapsto> Y \<rbrace>\<close> by simp
-lemma \<phi>M_tail_right: \<open>\<^bold>p\<^bold>r\<^bold>o\<^bold>c F \<lbrace> X \<longmapsto> 1 \<heavy_comma> Y \<rbrace> \<Longrightarrow> \<^bold>p\<^bold>r\<^bold>o\<^bold>c F \<lbrace> X \<longmapsto> Y \<rbrace>\<close> by simp
-lemma \<phi>M_tail_right_right: \<open>\<^bold>p\<^bold>r\<^bold>o\<^bold>c F \<lbrace> X \<longmapsto> Y\<heavy_comma> 1 \<rbrace> \<Longrightarrow> \<^bold>p\<^bold>r\<^bold>o\<^bold>c F \<lbrace> X \<longmapsto> Y \<rbrace>\<close> by simp
+lemma \<phi>M_tail_right: \<open>\<^bold>p\<^bold>r\<^bold>o\<^bold>c F \<lbrace> X \<longmapsto> \<lambda>v. 1 \<heavy_comma> Y v \<rbrace> \<Longrightarrow> \<^bold>p\<^bold>r\<^bold>o\<^bold>c F \<lbrace> X \<longmapsto> Y \<rbrace>\<close> by simp
+lemma \<phi>M_tail_right_right: \<open>\<^bold>p\<^bold>r\<^bold>o\<^bold>c F \<lbrace> X \<longmapsto> \<lambda>v. Y v\<heavy_comma> 1 \<rbrace> \<Longrightarrow> \<^bold>p\<^bold>r\<^bold>o\<^bold>c F \<lbrace> X \<longmapsto> Y \<rbrace>\<close> by simp
 lemma \<phi>M_detail_left[\<phi>reason 2200000]:  \<open>\<^bold>p\<^bold>r\<^bold>o\<^bold>c F \<lbrace> X \<longmapsto> Y \<rbrace> \<Longrightarrow> \<^bold>p\<^bold>r\<^bold>o\<^bold>c F \<lbrace> 1\<heavy_comma> X \<longmapsto> Y \<rbrace>\<close> by simp
-lemma \<phi>M_detail_right[\<phi>reason 2200000]: \<open>\<^bold>p\<^bold>r\<^bold>o\<^bold>c F \<lbrace> X \<longmapsto> Y \<rbrace> \<Longrightarrow> \<^bold>p\<^bold>r\<^bold>o\<^bold>c F \<lbrace> X \<longmapsto> 1\<heavy_comma> Y \<rbrace>\<close> by simp
+lemma \<phi>M_detail_right[\<phi>reason 2200000]: \<open>\<^bold>p\<^bold>r\<^bold>o\<^bold>c F \<lbrace> X \<longmapsto> Y \<rbrace> \<Longrightarrow> \<^bold>p\<^bold>r\<^bold>o\<^bold>c F \<lbrace> X \<longmapsto> \<lambda>v. 1\<heavy_comma> Y v \<rbrace>\<close> by simp
 
-lemma \<phi>M_get_Val[\<phi>reason!]:
-  \<open>(\<And>v. v \<in> A \<Longrightarrow> \<^bold>p\<^bold>r\<^bold>o\<^bold>c F v \<lbrace> X \<longmapsto> Y \<^bold>t\<^bold>h\<^bold>r\<^bold>o\<^bold>w\<^bold>s E \<rbrace> ) \<Longrightarrow> \<^bold>p\<^bold>r\<^bold>o\<^bold>c \<phi>M_get_Val F \<lbrace> X\<heavy_comma> VAL A \<longmapsto> Y \<^bold>t\<^bold>h\<^bold>r\<^bold>o\<^bold>w\<^bold>s E \<rbrace>\<close>
-  unfolding \<phi>Procedure_def \<phi>M_get_Val_def by (auto simp add: \<phi>expns times_list_def) blast
-
-lemmas [\<phi>reason!] = \<phi>M_tail_left[OF \<phi>M_get_Val]
-
-lemma \<phi>M_getV[\<phi>reason!]: \<open>(\<And>v. v \<in> A \<Longrightarrow> <\<phi>expn> v \<in> Well_Type TY)
-            \<Longrightarrow> (\<And>v. v \<in> A \<Longrightarrow> \<^bold>p\<^bold>r\<^bold>o\<^bold>c F (VDT_dest v) \<lbrace> X \<longmapsto> Y \<^bold>t\<^bold>h\<^bold>r\<^bold>o\<^bold>w\<^bold>s E \<rbrace> )
-            \<Longrightarrow> \<^bold>p\<^bold>r\<^bold>o\<^bold>c \<phi>M_getV TY VDT_dest F \<lbrace> X\<heavy_comma> VAL A \<longmapsto> Y \<^bold>t\<^bold>h\<^bold>r\<^bold>o\<^bold>w\<^bold>s E \<rbrace>\<close>
+lemma \<phi>M_getV[\<phi>reason!]: \<open>(v \<in> (x \<Ztypecolon> A) \<Longrightarrow> <\<phi>expn> v \<in> Well_Type TY)
+            \<Longrightarrow> (v \<in> (x \<Ztypecolon> A) \<Longrightarrow> \<^bold>p\<^bold>r\<^bold>o\<^bold>c F (VDT_dest v) \<lbrace> X \<longmapsto> Y \<^bold>t\<^bold>h\<^bold>r\<^bold>o\<^bold>w\<^bold>s E \<rbrace> )
+            \<Longrightarrow> \<^bold>p\<^bold>r\<^bold>o\<^bold>c \<phi>M_getV TY VDT_dest v F \<lbrace> X\<heavy_comma> x \<Ztypecolon> Val v A \<longmapsto> Y \<^bold>t\<^bold>h\<^bold>r\<^bold>o\<^bold>w\<^bold>s E \<rbrace>\<close>
   unfolding \<phi>M_getV_def Premise_def
-  by (rule \<phi>M_get_Val, rule \<phi>SEQ[where B = X], rule \<phi>CONSEQ'E, rule subty_0, rule \<phi>M_assert; blast)
+  by (clarsimp simp add: \<phi>expns)
 
-lemmas [\<phi>reason!] = \<phi>M_tail_left[OF \<phi>M_getV]
+declare \<phi>M_getV[THEN \<phi>M_tail_left, \<phi>reason!]
 
-lemma \<phi>M_put_Val[\<phi>reason! on \<open>\<^bold>p\<^bold>r\<^bold>o\<^bold>c \<phi>M_put_Val ?v \<lbrace> ?X \<longmapsto> ?Y \<rbrace>\<close>]:
-  \<open><\<phi>expn> v \<in> A \<Longrightarrow> \<^bold>p\<^bold>r\<^bold>o\<^bold>c \<phi>M_put_Val v \<lbrace> X \<longmapsto> X\<heavy_comma> VAL A \<rbrace>\<close>
-  unfolding \<phi>M_put_Val_def \<phi>Procedure_def Premise_def
-  by (simp add: \<phi>expns times_list_def) (metis append.left_neutral append_Cons) 
+lemma \<phi>M_Success[\<phi>reason!]:
+  \<open> <\<phi>expn> v \<in> (y \<Ztypecolon> T)
+\<Longrightarrow> \<^bold>p\<^bold>r\<^bold>o\<^bold>c Success v \<lbrace> X \<longmapsto> \<lambda>u. X\<heavy_comma> y \<Ztypecolon> Val u T \<rbrace> \<close>
+  unfolding \<phi>Procedure_def by (clarsimp simp add: \<phi>expns)
 
-lemmas [\<phi>reason 1500000 on \<open>\<^bold>p\<^bold>r\<^bold>o\<^bold>c \<phi>M_put_Val ?v \<lbrace> Void \<longmapsto> ?Y \<rbrace>\<close>]
-  = \<phi>M_tail_right[OF \<phi>M_put_Val]
+declare \<phi>M_Success[where X=1, simplified, \<phi>reason!]
 
 end
 
