NuLLReps.thy
@@ -458,9 +458,8 @@ lemma Var_subty:
 
 lemma Var_cast_\<phi>app[\<phi>overload cast]: 
   \<open> \<^bold>a\<^bold>r\<^bold>g\<^bold>u\<^bold>m\<^bold>e\<^bold>n\<^bold>t \<^bold>s\<^bold>u\<^bold>b\<^bold>t\<^bold>y\<^bold>p\<^bold>e x \<Ztypecolon> T \<longmapsto> x' \<Ztypecolon> T' \<^bold>w\<^bold>i\<^bold>t\<^bold>h P
-\<Longrightarrow> \<^bold>s\<^bold>u\<^bold>b\<^bold>t\<^bold>y\<^bold>p\<^bold>e FIX OBJ x \<Ztypecolon> Var vname T \<longmapsto> OBJ x' \<Ztypecolon> Var vname T' \<^bold>w\<^bold>i\<^bold>t\<^bold>h P\<close>
-  apply (rule cast_obj_\<phi>app)
-  unfolding Argument_def
+\<Longrightarrow> \<^bold>s\<^bold>u\<^bold>b\<^bold>t\<^bold>y\<^bold>p\<^bold>e FIX x \<Ztypecolon> Var vname T \<longmapsto> x' \<Ztypecolon> Var vname T' \<^bold>w\<^bold>i\<^bold>t\<^bold>h P\<close>
+  unfolding Argument_def Fix_def
   using Var_subty .
 
 lemma Var_ExTyp[simp]:
@@ -475,70 +474,49 @@ lemma [\<phi>reason 1200 on \<open>EqualAddress (?xa \<Ztypecolon> Var ?va ?Ta) 
   \<open>EqualAddress (xa \<Ztypecolon> Var var Ta) (xb \<Ztypecolon> Var var Tb)\<close>
   unfolding EqualAddress_def ..
 
-lemma [\<phi>reason 110 on \<open>\<^bold>s\<^bold>u\<^bold>b\<^bold>t\<^bold>y\<^bold>p\<^bold>e ?R \<heavy_comma> OBJ ?H \<longmapsto> ?R''' * \<blangle> OBJ ?X \<brangle> \<^bold>w\<^bold>i\<^bold>t\<^bold>h ?P \<^bold>@\<^bold>G\<^bold>O\<^bold>A\<^bold>L ?G\<close>]: \<comment> \<open>attempts the immediate cell\<close>
+lemma [\<phi>reason 110 on \<open>\<^bold>s\<^bold>u\<^bold>b\<^bold>t\<^bold>y\<^bold>p\<^bold>e ?R \<heavy_comma> ?H \<longmapsto> ?R''' * \<blangle> ?X \<brangle> \<^bold>w\<^bold>i\<^bold>t\<^bold>h ?P \<^bold>@\<^bold>G\<^bold>O\<^bold>A\<^bold>L ?G\<close>]: \<comment> \<open>attempts the immediate cell\<close>
   " CHK_SUBGOAL G
 \<Longrightarrow> \<^bold>s\<^bold>u\<^bold>b\<^bold>t\<^bold>y\<^bold>p\<^bold>e x \<Ztypecolon> T \<longmapsto> x' \<Ztypecolon> T' \<^bold>w\<^bold>i\<^bold>t\<^bold>h P
-\<Longrightarrow> \<^bold>s\<^bold>u\<^bold>b\<^bold>t\<^bold>y\<^bold>p\<^bold>e R\<heavy_comma> OBJ x \<Ztypecolon> Var var T \<longmapsto> R\<heavy_comma> \<blangle> OBJ x' \<Ztypecolon> Var var T' \<brangle> \<^bold>w\<^bold>i\<^bold>t\<^bold>h P \<^bold>@\<^bold>G\<^bold>O\<^bold>A\<^bold>L G"
+\<Longrightarrow> \<^bold>s\<^bold>u\<^bold>b\<^bold>t\<^bold>y\<^bold>p\<^bold>e R\<heavy_comma> x \<Ztypecolon> Var var T \<longmapsto> R\<heavy_comma> \<blangle> x' \<Ztypecolon> Var var T' \<brangle> \<^bold>w\<^bold>i\<^bold>t\<^bold>h P \<^bold>@\<^bold>G\<^bold>O\<^bold>A\<^bold>L G"
   unfolding cast_def
   by (simp add: \<phi>expns times_list_def, blast)
 
 
 subsubsection \<open>Synthesis Rules\<close>
 
-lemma [\<phi>reason on \<open>\<^bold>p\<^bold>r\<^bold>o\<^bold>c ?f \<lbrace> ?S1 \<longmapsto> ?S2\<heavy_comma> SYNTHESIS ?x \<Ztypecolon> Var ?var ?T \<^bold>t\<^bold>h\<^bold>r\<^bold>o\<^bold>w\<^bold>s ?E \<rbrace> \<^bold>@\<^bold>G\<^bold>O\<^bold>A\<^bold>L ?G\<close>]:
+lemma [\<phi>reason on \<open>\<^bold>p\<^bold>r\<^bold>o\<^bold>c ?f \<lbrace> ?S1 \<longmapsto> \<lambda>_. ?S2\<heavy_comma> SYNTHESIS ?x \<Ztypecolon> Var ?var ?T \<^bold>t\<^bold>h\<^bold>r\<^bold>o\<^bold>w\<^bold>s ?E \<rbrace> \<^bold>@\<^bold>G\<^bold>O\<^bold>A\<^bold>L ?G\<close>]:
   \<open> SUBGOAL G G'
-\<Longrightarrow> \<^bold>s\<^bold>u\<^bold>b\<^bold>t\<^bold>y\<^bold>p\<^bold>e S1 \<longmapsto> S2\<heavy_comma> \<blangle> OBJ x \<Ztypecolon> Var var T \<brangle> \<^bold>@\<^bold>G\<^bold>O\<^bold>A\<^bold>L G'
+\<Longrightarrow> \<^bold>s\<^bold>u\<^bold>b\<^bold>t\<^bold>y\<^bold>p\<^bold>e S1 \<longmapsto> S2\<heavy_comma> \<blangle> x \<Ztypecolon> Var var T \<brangle> \<^bold>@\<^bold>G\<^bold>O\<^bold>A\<^bold>L G'
 \<Longrightarrow> SOLVE_SUBGOAL G'
-\<Longrightarrow> \<^bold>p\<^bold>r\<^bold>o\<^bold>c EMPTY_PROC \<lbrace> S1 \<longmapsto> S2\<heavy_comma> SYNTHESIS x \<Ztypecolon> Var var T \<rbrace> \<^bold>@\<^bold>G\<^bold>O\<^bold>A\<^bold>L G\<close>
+\<Longrightarrow> \<^bold>p\<^bold>r\<^bold>o\<^bold>c Success () \<lbrace> S1 \<longmapsto> \<lambda>_. S2\<heavy_comma> SYNTHESIS x \<Ztypecolon> Var var T \<rbrace> \<^bold>@\<^bold>G\<^bold>O\<^bold>A\<^bold>L G\<close>
   unfolding GOAL_CTXT_def FOCUS_TAG_def Synthesis_def
-  using "\<phi>cast" \<phi>reassemble_proc_0 \<phi>reassemble_proc_final
-  by metis
+  using "\<phi>cast" \<phi>reassemble_proc_final
+  by (metis (no_types, lifting) \<phi>SKIP \<phi>apply_proc)
 
 
 subsubsection \<open>Application Methods for Subtyping\<close>
 
 lemma [\<phi>reason 2000 on \<open>
-  PROP \<phi>Application_Method (Trueprop (\<^bold>s\<^bold>u\<^bold>b\<^bold>t\<^bold>y\<^bold>p\<^bold>e ?x \<Ztypecolon> ?T \<longmapsto> ?Y \<Ztypecolon> ?U \<^bold>w\<^bold>i\<^bold>t\<^bold>h ?P))
-            (Trueprop (\<^bold>c\<^bold>u\<^bold>r\<^bold>r\<^bold>e\<^bold>n\<^bold>t ?blk [?RR] \<^bold>r\<^bold>e\<^bold>s\<^bold>u\<^bold>l\<^bold>t\<^bold>s \<^bold>i\<^bold>n OBJ ?x \<Ztypecolon> Var ?var ?T)) ?Result
-\<close>]:
-  \<open> PROP \<phi>Application_Success
-\<Longrightarrow> PROP \<phi>Application_Method (Trueprop (\<^bold>s\<^bold>u\<^bold>b\<^bold>t\<^bold>y\<^bold>p\<^bold>e x \<Ztypecolon> T \<longmapsto> x \<Ztypecolon> U \<^bold>w\<^bold>i\<^bold>t\<^bold>h P))
-      (Trueprop (\<^bold>c\<^bold>u\<^bold>r\<^bold>r\<^bold>e\<^bold>n\<^bold>t blk [RR] \<^bold>r\<^bold>e\<^bold>s\<^bold>u\<^bold>l\<^bold>t\<^bold>s \<^bold>i\<^bold>n OBJ x \<Ztypecolon> Var var T))
-      (Trueprop ((\<^bold>c\<^bold>u\<^bold>r\<^bold>r\<^bold>e\<^bold>n\<^bold>t blk [RR] \<^bold>r\<^bold>e\<^bold>s\<^bold>u\<^bold>l\<^bold>t\<^bold>s \<^bold>i\<^bold>n OBJ x \<Ztypecolon> Var var U) \<and> P))\<close>
-  unfolding \<phi>Application_Method_def \<phi>Application_def
-  using "\<phi>cast_P" Var_cast_\<phi>app[unfolded Argument_def Fix_def] by metis
-
-lemma [\<phi>reason 2000 on \<open>
-  PROP \<phi>Application_Method (Trueprop (\<^bold>s\<^bold>u\<^bold>b\<^bold>t\<^bold>y\<^bold>p\<^bold>e ?x' \<Ztypecolon> ?T' \<longmapsto> ?y \<Ztypecolon> ?U \<^bold>w\<^bold>i\<^bold>t\<^bold>h ?P))
-            (Trueprop (\<^bold>c\<^bold>u\<^bold>r\<^bold>r\<^bold>e\<^bold>n\<^bold>t ?blk [?RR] \<^bold>r\<^bold>e\<^bold>s\<^bold>u\<^bold>l\<^bold>t\<^bold>s \<^bold>i\<^bold>n OBJ ?x \<Ztypecolon> Var ?var ?T)) ?Result
-\<close>]:
-  \<open> SUBGOAL TOP_GOAL G
-\<Longrightarrow> \<^bold>s\<^bold>u\<^bold>b\<^bold>t\<^bold>y\<^bold>p\<^bold>e x \<Ztypecolon> T \<longmapsto> x' \<Ztypecolon> T' \<^bold>w\<^bold>i\<^bold>t\<^bold>h Any
-\<Longrightarrow> SOLVE_SUBGOAL G
-\<Longrightarrow> PROP \<phi>Application_Success
-\<Longrightarrow> \<^bold>o\<^bold>b\<^bold>l\<^bold>i\<^bold>g\<^bold>a\<^bold>t\<^bold>i\<^bold>o\<^bold>n True
-\<Longrightarrow> PROP \<phi>Application_Method (Trueprop (\<^bold>s\<^bold>u\<^bold>b\<^bold>t\<^bold>y\<^bold>p\<^bold>e x' \<Ztypecolon> T' \<longmapsto> y \<Ztypecolon> U \<^bold>w\<^bold>i\<^bold>t\<^bold>h P))
-      (Trueprop (\<^bold>c\<^bold>u\<^bold>r\<^bold>r\<^bold>e\<^bold>n\<^bold>t blk [RR] \<^bold>r\<^bold>e\<^bold>s\<^bold>u\<^bold>l\<^bold>t\<^bold>s \<^bold>i\<^bold>n OBJ x \<Ztypecolon> Var var T))
-      (Trueprop ((\<^bold>c\<^bold>u\<^bold>r\<^bold>r\<^bold>e\<^bold>n\<^bold>t blk [RR] \<^bold>r\<^bold>e\<^bold>s\<^bold>u\<^bold>l\<^bold>t\<^bold>s \<^bold>i\<^bold>n OBJ y \<Ztypecolon> Var var U) \<and> P))\<close>
-  unfolding \<phi>Application_Method_def \<phi>Application_def
-  using "\<phi>cast_P" Var_cast_\<phi>app[unfolded Argument_def Fix_def] by metis
-
-
-lemma [\<phi>reason 2000 on \<open>
   PROP \<phi>Application_Method (Trueprop (\<^bold>s\<^bold>u\<^bold>b\<^bold>t\<^bold>y\<^bold>p\<^bold>e ?x \<Ztypecolon> ?T \<longmapsto> ?y \<Ztypecolon> ?U \<^bold>w\<^bold>i\<^bold>t\<^bold>h ?P))
-          (Trueprop (\<^bold>c\<^bold>u\<^bold>r\<^bold>r\<^bold>e\<^bold>n\<^bold>t ?blk [?RR] \<^bold>r\<^bold>e\<^bold>s\<^bold>u\<^bold>l\<^bold>t\<^bold>s \<^bold>i\<^bold>n ?R\<heavy_comma> OBJ ?x \<Ztypecolon> Var ?var ?T)) ?Result
+          (Trueprop (\<^bold>c\<^bold>u\<^bold>r\<^bold>r\<^bold>e\<^bold>n\<^bold>t ?blk [?RR] \<^bold>r\<^bold>e\<^bold>s\<^bold>u\<^bold>l\<^bold>t\<^bold>s \<^bold>i\<^bold>n ?R\<heavy_comma> ?x \<Ztypecolon> Var ?var ?T)) ?Result
+\<close> if no \<open>
+  PROP \<phi>Application_Method (Trueprop (\<^bold>s\<^bold>u\<^bold>b\<^bold>t\<^bold>y\<^bold>p\<^bold>e ?x \<Ztypecolon> Var ?var ?T \<longmapsto> ?y \<Ztypecolon> ?U \<^bold>w\<^bold>i\<^bold>t\<^bold>h ?P))
+          (Trueprop (\<^bold>c\<^bold>u\<^bold>r\<^bold>r\<^bold>e\<^bold>n\<^bold>t ?blk [?RR] \<^bold>r\<^bold>e\<^bold>s\<^bold>u\<^bold>l\<^bold>t\<^bold>s \<^bold>i\<^bold>n ?R)) ?Result
 \<close>]:
   \<open> PROP \<phi>Application_Success
 \<Longrightarrow> PROP \<phi>Application_Method (Trueprop (\<^bold>s\<^bold>u\<^bold>b\<^bold>t\<^bold>y\<^bold>p\<^bold>e x \<Ztypecolon> T \<longmapsto> y \<Ztypecolon> U \<^bold>w\<^bold>i\<^bold>t\<^bold>h P))
-      (Trueprop (\<^bold>c\<^bold>u\<^bold>r\<^bold>r\<^bold>e\<^bold>n\<^bold>t blk [RR] \<^bold>r\<^bold>e\<^bold>s\<^bold>u\<^bold>l\<^bold>t\<^bold>s \<^bold>i\<^bold>n R\<heavy_comma> OBJ x \<Ztypecolon> Var var T))
-      (Trueprop ((\<^bold>c\<^bold>u\<^bold>r\<^bold>r\<^bold>e\<^bold>n\<^bold>t blk [RR] \<^bold>r\<^bold>e\<^bold>s\<^bold>u\<^bold>l\<^bold>t\<^bold>s \<^bold>i\<^bold>n R\<heavy_comma> OBJ y \<Ztypecolon> Var var U) \<and> P))\<close>
+      (Trueprop (\<^bold>c\<^bold>u\<^bold>r\<^bold>r\<^bold>e\<^bold>n\<^bold>t blk [RR] \<^bold>r\<^bold>e\<^bold>s\<^bold>u\<^bold>l\<^bold>t\<^bold>s \<^bold>i\<^bold>n R\<heavy_comma> x \<Ztypecolon> Var var T))
+      (Trueprop ((\<^bold>c\<^bold>u\<^bold>r\<^bold>r\<^bold>e\<^bold>n\<^bold>t blk [RR] \<^bold>r\<^bold>e\<^bold>s\<^bold>u\<^bold>l\<^bold>t\<^bold>s \<^bold>i\<^bold>n R\<heavy_comma> y \<Ztypecolon> Var var U) \<and> P))\<close>
   unfolding \<phi>Application_Method_def \<phi>Application_def
   using "\<phi>cast_P" Var_cast_\<phi>app[unfolded Argument_def Fix_def] \<phi>cast_intro_frame by metis
 
 
 lemma [\<phi>reason 2000 on \<open>
   PROP \<phi>Application_Method (Trueprop (\<^bold>s\<^bold>u\<^bold>b\<^bold>t\<^bold>y\<^bold>p\<^bold>e ?x' \<Ztypecolon> ?T' \<longmapsto> ?y \<Ztypecolon> ?U \<^bold>w\<^bold>i\<^bold>t\<^bold>h ?P))
-      (Trueprop (\<^bold>c\<^bold>u\<^bold>r\<^bold>r\<^bold>e\<^bold>n\<^bold>t ?blk [?RR] \<^bold>r\<^bold>e\<^bold>s\<^bold>u\<^bold>l\<^bold>t\<^bold>s \<^bold>i\<^bold>n ?R\<heavy_comma> OBJ ?x \<Ztypecolon> Var ?var ?T)) ?Result
+      (Trueprop (\<^bold>c\<^bold>u\<^bold>r\<^bold>r\<^bold>e\<^bold>n\<^bold>t ?blk [?RR] \<^bold>r\<^bold>e\<^bold>s\<^bold>u\<^bold>l\<^bold>t\<^bold>s \<^bold>i\<^bold>n ?R\<heavy_comma> ?x \<Ztypecolon> Var ?var ?T)) ?Result
+\<close> if no \<open>
+  PROP \<phi>Application_Method (Trueprop (\<^bold>s\<^bold>u\<^bold>b\<^bold>t\<^bold>y\<^bold>p\<^bold>e ?x \<Ztypecolon> Var ?var ?T \<longmapsto> ?y \<Ztypecolon> ?U \<^bold>w\<^bold>i\<^bold>t\<^bold>h ?P))
+          (Trueprop (\<^bold>c\<^bold>u\<^bold>r\<^bold>r\<^bold>e\<^bold>n\<^bold>t ?blk [?RR] \<^bold>r\<^bold>e\<^bold>s\<^bold>u\<^bold>l\<^bold>t\<^bold>s \<^bold>i\<^bold>n ?R)) ?Result
 \<close>]:
   \<open> SUBGOAL TOP_GOAL G
 \<Longrightarrow> \<^bold>s\<^bold>u\<^bold>b\<^bold>t\<^bold>y\<^bold>p\<^bold>e x \<Ztypecolon> T \<longmapsto> x' \<Ztypecolon> T' \<^bold>w\<^bold>i\<^bold>t\<^bold>h Any
@@ -546,8 +524,8 @@ lemma [\<phi>reason 2000 on \<open>
 \<Longrightarrow> PROP \<phi>Application_Success
 \<Longrightarrow> \<^bold>o\<^bold>b\<^bold>l\<^bold>i\<^bold>g\<^bold>a\<^bold>t\<^bold>i\<^bold>o\<^bold>n True
 \<Longrightarrow> PROP \<phi>Application_Method (Trueprop (\<^bold>s\<^bold>u\<^bold>b\<^bold>t\<^bold>y\<^bold>p\<^bold>e x' \<Ztypecolon> T' \<longmapsto> y \<Ztypecolon> U \<^bold>w\<^bold>i\<^bold>t\<^bold>h P))
-      (Trueprop (\<^bold>c\<^bold>u\<^bold>r\<^bold>r\<^bold>e\<^bold>n\<^bold>t blk [RR] \<^bold>r\<^bold>e\<^bold>s\<^bold>u\<^bold>l\<^bold>t\<^bold>s \<^bold>i\<^bold>n R\<heavy_comma> OBJ x \<Ztypecolon> Var var T))
-      (Trueprop ((\<^bold>c\<^bold>u\<^bold>r\<^bold>r\<^bold>e\<^bold>n\<^bold>t blk [RR] \<^bold>r\<^bold>e\<^bold>s\<^bold>u\<^bold>l\<^bold>t\<^bold>s \<^bold>i\<^bold>n R\<heavy_comma> OBJ y \<Ztypecolon> Var var U) \<and> P))\<close>
+      (Trueprop (\<^bold>c\<^bold>u\<^bold>r\<^bold>r\<^bold>e\<^bold>n\<^bold>t blk [RR] \<^bold>r\<^bold>e\<^bold>s\<^bold>u\<^bold>l\<^bold>t\<^bold>s \<^bold>i\<^bold>n R\<heavy_comma> x \<Ztypecolon> Var var T))
+      (Trueprop ((\<^bold>c\<^bold>u\<^bold>r\<^bold>r\<^bold>e\<^bold>n\<^bold>t blk [RR] \<^bold>r\<^bold>e\<^bold>s\<^bold>u\<^bold>l\<^bold>t\<^bold>s \<^bold>i\<^bold>n R\<heavy_comma> y \<Ztypecolon> Var var U) \<and> P))\<close>
   unfolding \<phi>Application_Method_def \<phi>Application_def
   using "\<phi>cast_P" Var_cast_\<phi>app[unfolded Argument_def Fix_def] \<phi>cast_intro_frame by metis
 
