NuStd_Base.thy
@@ -25,12 +25,6 @@ declare Nat.One_nat_def[simp del] Num.add_2_eq_Suc'[simp del] split_paired_All[s
 
 section \<open>Basic Operations\<close>
 
-subsection \<open>Manipulation of the Op-Stack\<close>
-
-lemma (in std) op_drop:
-  \<open>\<^bold>p\<^bold>r\<^bold>o\<^bold>c op_drop \<lbrace> VAL X \<longmapsto> Void \<rbrace>\<close>
-  unfolding op_drop_def by \<phi>reason
-
 subsection \<open>Variable\<close>
 
 subsubsection \<open>Syntax\<close>
@@ -58,7 +52,7 @@ definition Set_Variable :: \<open>varname \<Rightarrow> 'a \<Rightarrow> 'a\<clo
   where [iff]: \<open>($x := y) = y\<close>
 
 lemma (in std) [\<phi>reason 2000 on \<open>Synthesis_Parse (?var::varname) ?Y\<close>]:
-  \<open>Synthesis_Parse var (OBJ x \<Ztypecolon> Var var T)\<close>
+  \<open>Synthesis_Parse var (\<lambda>_. x \<Ztypecolon> Var var T)\<close>
   unfolding Synthesis_Parse_def ..
 
 
@@ -88,43 +82,45 @@ declare [ [\<phi>not_define_new_const] ]
 proc op_get_var:
   assumes [unfolded \<phi>SemType_def subset_iff, useful]: \<open>\<phi>SemType (x \<Ztypecolon> T) TY\<close>
   argument \<open>x \<Ztypecolon> Var vname T\<close>
-  return   \<open>x \<Ztypecolon> Var vname T\<heavy_comma> x \<Ztypecolon> T\<close>
+  return   \<open>x \<Ztypecolon> Var vname T\<heavy_comma> x \<Ztypecolon> \<^bold>v\<^bold>a\<^bold>l T\<close>
   \<medium_left_bracket>
     to_Identity op_get_var''
   \<medium_right_bracket>. .
 
-lemma [\<phi>reason on \<open>\<^bold>p\<^bold>r\<^bold>o\<^bold>c ?f \<lbrace> ?R \<longmapsto> ?R'\<heavy_comma> SYNTHESIS VAL ?x <val-of-var> ?var \<Ztypecolon> ?T \<^bold>t\<^bold>h\<^bold>r\<^bold>o\<^bold>w\<^bold>s ?E \<rbrace> \<^bold>@\<^bold>G\<^bold>O\<^bold>A\<^bold>L ?G\<close>]:
+lemma [\<phi>reason on \<open>\<^bold>p\<^bold>r\<^bold>o\<^bold>c ?f \<lbrace> ?R \<longmapsto> ?R'\<heavy_comma> SYNTHESIS ?x <val-of-var> ?var \<Ztypecolon> \<^bold>v\<^bold>a\<^bold>l ?T \<^bold>t\<^bold>h\<^bold>r\<^bold>o\<^bold>w\<^bold>s ?E \<rbrace> \<^bold>@\<^bold>G\<^bold>O\<^bold>A\<^bold>L ?G\<close>]:
   \<open> SUBGOAL G G2
-\<Longrightarrow> \<^bold>s\<^bold>u\<^bold>b\<^bold>t\<^bold>y\<^bold>p\<^bold>e X \<longmapsto> Y\<heavy_comma> \<blangle> OBJ x \<Ztypecolon> Var var T \<brangle> \<^bold>@\<^bold>G\<^bold>O\<^bold>A\<^bold>L G2
+\<Longrightarrow> \<^bold>s\<^bold>u\<^bold>b\<^bold>t\<^bold>y\<^bold>p\<^bold>e X \<longmapsto> Y\<heavy_comma> \<blangle> x \<Ztypecolon> Var var T \<brangle> \<^bold>@\<^bold>G\<^bold>O\<^bold>A\<^bold>L G2
 \<Longrightarrow> SOLVE_SUBGOAL G2
 \<Longrightarrow> \<phi>SemType (x \<Ztypecolon> T) TY
-\<Longrightarrow> \<^bold>p\<^bold>r\<^bold>o\<^bold>c op_get_var var TY \<lbrace> X \<longmapsto> Y\<heavy_comma> OBJ x \<Ztypecolon> Var var T \<heavy_comma> SYNTHESIS x <val-of-var> var \<Ztypecolon> T \<rbrace> \<^bold>@\<^bold>G\<^bold>O\<^bold>A\<^bold>L G\<close>
+\<Longrightarrow> \<^bold>p\<^bold>r\<^bold>o\<^bold>c op_get_var var TY \<lbrace> X \<longmapsto> Y\<heavy_comma> x \<Ztypecolon> Var var T \<heavy_comma> SYNTHESIS x <val-of-var> var \<Ztypecolon> \<^bold>v\<^bold>a\<^bold>l T \<rbrace> \<^bold>@\<^bold>G\<^bold>O\<^bold>A\<^bold>L G\<close>
   \<medium_left_bracket> premises _ and GetVar and _ and [\<phi>reason on \<open>\<phi>SemType (x \<Ztypecolon> T) ?TY\<close>]
     GetVar op_get_var \<medium_right_bracket>. .
 
 
 paragraph \<open>Set Variable\<close>
 
+declare [ [\<phi>trace_reasoning]]
+
 proc op_set_var:
   assumes [unfolded \<phi>SemType_def subset_iff, useful]: \<open>\<phi>SemType (x \<Ztypecolon> T) TY\<close>
   assumes [unfolded \<phi>SemType_def subset_iff, useful]: \<open>\<phi>SemType (y \<Ztypecolon> U) TY\<close>
-  argument \<open>x \<Ztypecolon> Var var T\<heavy_comma> y \<Ztypecolon> U\<close>
+  argument \<open>x \<Ztypecolon> Var var T\<heavy_comma> y \<Ztypecolon> \<^bold>v\<^bold>a\<^bold>l U\<close>
   return   \<open>y \<Ztypecolon> Var var U\<close>
-  \<medium_left_bracket> to_Identity \<open>var\<close> to_Identity op_set_var'' \<medium_right_bracket>. .
+  \<medium_left_bracket> ;; to_Identity ;; \<open>var\<close> ;; to_Identity ;; op_set_var'' \<medium_right_bracket>. .
 
 proc op_set_var__synthesis[
-  \<phi>reason on \<open>\<^bold>p\<^bold>r\<^bold>o\<^bold>c ?f \<lbrace> ?R \<longmapsto> ?R'\<heavy_comma> SYNTHESIS VAL ($?var := ?y) \<Ztypecolon> ?U \<^bold>t\<^bold>h\<^bold>r\<^bold>o\<^bold>w\<^bold>s ?E \<rbrace> \<^bold>@\<^bold>G\<^bold>O\<^bold>A\<^bold>L ?G\<close>
+  \<phi>reason on \<open>\<^bold>p\<^bold>r\<^bold>o\<^bold>c ?f \<lbrace> ?R \<longmapsto> ?R'\<heavy_comma> SYNTHESIS ($?var := ?y) \<Ztypecolon> \<^bold>v\<^bold>a\<^bold>l ?U \<^bold>t\<^bold>h\<^bold>r\<^bold>o\<^bold>w\<^bold>s ?E \<rbrace> \<^bold>@\<^bold>G\<^bold>O\<^bold>A\<^bold>L ?G\<close>
 ]:
-assumes G: \<open>\<^bold>p\<^bold>r\<^bold>o\<^bold>c g \<lbrace> X \<longmapsto> X1\<heavy_comma> SYNTHESIS VAL y \<Ztypecolon> U \<^bold>t\<^bold>h\<^bold>r\<^bold>o\<^bold>w\<^bold>s E\<rbrace> \<^bold>@\<^bold>G\<^bold>O\<^bold>A\<^bold>L G \<close>
+assumes G: \<open>\<^bold>p\<^bold>r\<^bold>o\<^bold>c g \<lbrace> X \<longmapsto> X1\<heavy_comma> SYNTHESIS y \<Ztypecolon> \<^bold>v\<^bold>a\<^bold>l U \<^bold>t\<^bold>h\<^bold>r\<^bold>o\<^bold>w\<^bold>s E\<rbrace> \<^bold>@\<^bold>G\<^bold>O\<^bold>A\<^bold>L G \<close>
   and      \<open>SUBGOAL G G2\<close>
   and S[unfolded GOAL_CTXT_def FOCUS_TAG_def]:
-        \<open>\<^bold>s\<^bold>u\<^bold>b\<^bold>t\<^bold>y\<^bold>p\<^bold>e X1\<heavy_comma> VAL y \<Ztypecolon> U \<longmapsto> \<blangle> Y\<heavy_comma> x \<Ztypecolon> Var var T\<heavy_comma> VAL y \<Ztypecolon> U \<brangle> \<^bold>w\<^bold>i\<^bold>t\<^bold>h Any \<^bold>@\<^bold>G\<^bold>O\<^bold>A\<^bold>L G2\<close>
+        \<open>\<And>vy. \<^bold>s\<^bold>u\<^bold>b\<^bold>t\<^bold>y\<^bold>p\<^bold>e X1\<heavy_comma> y \<Ztypecolon> Val vy U \<longmapsto> \<blangle> Y\<heavy_comma> x \<Ztypecolon> Var var T\<heavy_comma> y \<Ztypecolon> Val vy U \<brangle> \<^bold>w\<^bold>i\<^bold>t\<^bold>h Any \<^bold>@\<^bold>G\<^bold>O\<^bold>A\<^bold>L G2\<close>
   and   \<open>SOLVE_SUBGOAL G2\<close>
   and [\<phi>reason on \<open>\<phi>SemType (x \<Ztypecolon> T) ?TY\<close>]: \<open>\<phi>SemType (x \<Ztypecolon> T) TY\<close>
   and [\<phi>reason on \<open>\<phi>SemType (y \<Ztypecolon> U) ?TY\<close>]: \<open>\<phi>SemType (y \<Ztypecolon> U) TY\<close>
  goal G
 argument \<open>X\<close>
-return   \<open>Y\<heavy_comma> y \<Ztypecolon> Var var U \<heavy_comma> SYNTHESIS ($var := y) \<Ztypecolon> U\<close>
+return   \<open>Y\<heavy_comma> y \<Ztypecolon> Var var U \<heavy_comma> SYNTHESIS ($var := y) \<Ztypecolon> \<^bold>v\<^bold>a\<^bold>l U\<close>
 throws   E
   \<medium_left_bracket> G S op_set_var op_get_var \<medium_right_bracket>. .
 
@@ -134,28 +130,32 @@ paragraph \<open>Declare New Variables\<close>
 
 proc (in std) op_var_scope:
   assumes [unfolded \<phi>SemType_def subset_iff, useful]: \<open>\<phi>SemType (x \<Ztypecolon> T) TY\<close>
-    and BLK: \<open>\<forall>var. \<^bold>p\<^bold>r\<^bold>o\<^bold>c F var \<lbrace> X\<heavy_comma> x \<Ztypecolon> Var var T \<longmapsto> Y\<heavy_comma> y \<Ztypecolon> Var var (U <of-type> TY) \<^bold>t\<^bold>h\<^bold>r\<^bold>o\<^bold>w\<^bold>s E\<heavy_comma> y \<Ztypecolon> Var var (U <of-type> TY) \<rbrace>\<close>
-  argument \<open>X\<heavy_comma> x \<Ztypecolon> T\<close>
+    and BLK: \<open>\<forall>var. \<^bold>p\<^bold>r\<^bold>o\<^bold>c F var \<lbrace> X\<heavy_comma> x \<Ztypecolon> Var var T \<longmapsto> \<lambda>ret. Y ret\<heavy_comma> y \<Ztypecolon> Var var (U <of-type> TY) \<^bold>t\<^bold>h\<^bold>r\<^bold>o\<^bold>w\<^bold>s E\<heavy_comma> y \<Ztypecolon> Var var (U <of-type> TY) \<rbrace>\<close>
+  argument \<open>X\<heavy_comma> x \<Ztypecolon> \<^bold>v\<^bold>a\<^bold>l T\<close>
   return   \<open>Y\<close>
   throws   E
   \<medium_left_bracket> to_Identity op_var_scope';;
-  note [ [\<phi>trace_reasoning] ] ;;
-    try'' \<medium_left_bracket> BLK to_Identity op_free_var \<medium_right_bracket>. \<medium_left_bracket> to_Identity op_free_var throw \<medium_right_bracket>. \<medium_right_bracket>. .
+    try'' \<medium_left_bracket> BLK to_Identity op_free_var \<medium_right_bracket>. \<medium_left_bracket> to_Identity op_free_var throw \<medium_right_bracket> .. \<medium_right_bracket>. .
+
+lemma \<open>(A\<heavy_comma> B) = (B \<heavy_comma>A)\<close>
+  by (simp add: mult.commute) 
 
 lemma "__\<phi>op_var_scope__":
   \<open> (\<And>var. \<^bold>p\<^bold>r\<^bold>o\<^bold>c F var \<lbrace> R\<heavy_comma> x \<Ztypecolon> Var var T\<heavy_comma>  X \<longmapsto> Y \<heavy_comma> y \<Ztypecolon> Var var (U <of-type> TY) \<^bold>t\<^bold>h\<^bold>r\<^bold>o\<^bold>w\<^bold>s E\<heavy_comma> y \<Ztypecolon> Var var (U <of-type> TY) \<rbrace>)
 \<Longrightarrow> \<phi>SemType (x \<Ztypecolon> T) TY
-\<Longrightarrow> \<^bold>p\<^bold>r\<^bold>o\<^bold>c op_var_scope TY F \<lbrace> R\<heavy_comma> (X\<heavy_comma> x \<Ztypecolon> T) \<longmapsto> Y \<^bold>t\<^bold>h\<^bold>r\<^bold>o\<^bold>w\<^bold>s E \<rbrace>\<close>
-  using op_var_scope_\<phi>app
-  by (smt (z3) OBJ_comm mult.assoc)
+\<Longrightarrow> \<^bold>p\<^bold>r\<^bold>o\<^bold>c op_var_scope TY raw F \<lbrace> R\<heavy_comma> (X\<heavy_comma> x \<Ztypecolon> Val raw T) \<longmapsto> \<lambda>_::unit. Y \<^bold>t\<^bold>h\<^bold>r\<^bold>o\<^bold>w\<^bold>s E \<rbrace>\<close>
+  unfolding mult.assoc[symmetric]
+  using op_var_scope_\<phi>app[where X=\<open>R\<heavy_comma> X\<close> and x = x and T = T and TY = TY and F=F and y=y, of Y U E raw]
+  by (smt (verit, best) ab_semigroup_mult_class.mult_ac(1) mult.commute)
 
 lemma "__\<phi>op_set_var__":
   \<open> \<^bold>p\<^bold>r\<^bold>o\<^bold>c g \<lbrace> R\<heavy_comma> y \<Ztypecolon> Var var U\<heavy_comma> X \<longmapsto> Z \<^bold>t\<^bold>h\<^bold>r\<^bold>o\<^bold>w\<^bold>s E \<rbrace>
 \<Longrightarrow> \<phi>SemType (x \<Ztypecolon> T) TY
 \<Longrightarrow> \<phi>SemType (y \<Ztypecolon> U) TY
-\<Longrightarrow> \<^bold>p\<^bold>r\<^bold>o\<^bold>c (op_set_var var TY \<ggreater> g) \<lbrace> R\<heavy_comma> (X\<heavy_comma> x \<Ztypecolon> Var var T \<heavy_comma> y \<Ztypecolon> U) \<longmapsto> Z \<^bold>t\<^bold>h\<^bold>r\<^bold>o\<^bold>w\<^bold>s E \<rbrace>\<close>
+\<Longrightarrow> \<^bold>p\<^bold>r\<^bold>o\<^bold>c (op_set_var var TY raw \<ggreater> g) \<lbrace> R\<heavy_comma> (X\<heavy_comma> x \<Ztypecolon> Var var T \<heavy_comma> y \<Ztypecolon> Val raw U) \<longmapsto> Z \<^bold>t\<^bold>h\<^bold>r\<^bold>o\<^bold>w\<^bold>s E \<rbrace>\<close>
   \<medium_left_bracket> premises G and [\<phi>reason on \<open>\<phi>SemType (x \<Ztypecolon> T) ?TY\<close>] and [\<phi>reason on \<open>\<phi>SemType (y \<Ztypecolon> U) ?TY\<close>]
     op_set_var G \<medium_right_bracket>. .
+
 
 
 lemma "__\<phi>op_var_scope__0":
@@ -182,48 +182,48 @@ subsubsection \<open>Boolean Arithmetic\<close>
 paragraph \<open>Not\<close>
 
 lemma (in std) op_not[\<phi>overload \<not>]:
-  \<open>\<^bold>p\<^bold>r\<^bold>o\<^bold>c op_not \<lbrace> x \<Ztypecolon> \<bool> \<longmapsto> \<not> x \<Ztypecolon> \<bool> \<rbrace>\<close>
+  \<open>\<^bold>p\<^bold>r\<^bold>o\<^bold>c op_not raw \<lbrace> x \<Ztypecolon> Val raw \<bool> \<longmapsto> \<not> x \<Ztypecolon> \<^bold>v\<^bold>a\<^bold>l \<bool> \<rbrace>\<close>
   unfolding op_not_def
   by \<phi>reason
 
 proc [
-    \<phi>reason on \<open>\<^bold>p\<^bold>r\<^bold>o\<^bold>c ?F \<lbrace> ?R \<longmapsto> ?R1\<heavy_comma> SYNTHESIS VAL \<not>?b \<Ztypecolon> ?T \<^bold>t\<^bold>h\<^bold>r\<^bold>o\<^bold>w\<^bold>s ?E \<rbrace> \<^bold>@\<^bold>G\<^bold>O\<^bold>A\<^bold>L ?G\<close>
+    \<phi>reason on \<open>\<^bold>p\<^bold>r\<^bold>o\<^bold>c ?F \<lbrace> ?R \<longmapsto> ?R1\<heavy_comma> SYNTHESIS \<not>?b \<Ztypecolon> Val ?v ?T \<^bold>t\<^bold>h\<^bold>r\<^bold>o\<^bold>w\<^bold>s ?E \<rbrace> \<^bold>@\<^bold>G\<^bold>O\<^bold>A\<^bold>L ?G\<close>
 ]:
-  assumes F1: \<open>\<^bold>p\<^bold>r\<^bold>o\<^bold>c f \<lbrace> R \<longmapsto> R1\<heavy_comma> SYNTHESIS b \<Ztypecolon> \<bool> \<rbrace>  \<^bold>@\<^bold>G\<^bold>O\<^bold>A\<^bold>L G\<close>
+  assumes F1: \<open>\<^bold>p\<^bold>r\<^bold>o\<^bold>c f \<lbrace> R \<longmapsto> R1\<heavy_comma> SYNTHESIS b \<Ztypecolon> \<^bold>v\<^bold>a\<^bold>l \<bool> \<rbrace>  \<^bold>@\<^bold>G\<^bold>O\<^bold>A\<^bold>L G\<close>
   goal G
   argument \<open>R\<close>
-  return   \<open>R1\<heavy_comma> SYNTHESIS VAL \<not>b \<Ztypecolon> \<bool>\<close>
+  return   \<open>R1\<heavy_comma> SYNTHESIS \<not>b \<Ztypecolon> \<^bold>v\<^bold>a\<^bold>l \<bool>\<close>
   \<medium_left_bracket> F1 \<not> \<medium_right_bracket>. .
 
 paragraph \<open>And\<close>
 
 lemma (in std) op_and[\<phi>overload \<and>]:
-  \<open>\<^bold>p\<^bold>r\<^bold>o\<^bold>c op_and \<lbrace> a \<Ztypecolon> \<bool>\<heavy_comma> b \<Ztypecolon> \<bool> \<longmapsto> a \<and> b \<Ztypecolon> \<bool> \<rbrace>\<close>
+  \<open>\<^bold>p\<^bold>r\<^bold>o\<^bold>c op_and vb va \<lbrace> a \<Ztypecolon> Val va \<bool>\<heavy_comma> b \<Ztypecolon> Val vb \<bool> \<longmapsto> a \<and> b \<Ztypecolon> \<^bold>v\<^bold>a\<^bold>l \<bool> \<rbrace>\<close>
   unfolding op_and_def
   by \<phi>reason
 
 proc [
-    \<phi>reason on \<open>\<^bold>p\<^bold>r\<^bold>o\<^bold>c ?F \<lbrace> ?R \<longmapsto> ?R2\<heavy_comma> SYNTHESIS VAL (?x \<and> ?y) \<Ztypecolon> ?T \<^bold>t\<^bold>h\<^bold>r\<^bold>o\<^bold>w\<^bold>s ?E \<rbrace> \<^bold>@\<^bold>G\<^bold>O\<^bold>A\<^bold>L ?G\<close>
+    \<phi>reason on \<open>\<^bold>p\<^bold>r\<^bold>o\<^bold>c ?F \<lbrace> ?R \<longmapsto> ?R2\<heavy_comma> SYNTHESIS (?x \<and> ?y) \<Ztypecolon> \<^bold>v\<^bold>a\<^bold>l ?T \<^bold>t\<^bold>h\<^bold>r\<^bold>o\<^bold>w\<^bold>s ?E \<rbrace> \<^bold>@\<^bold>G\<^bold>O\<^bold>A\<^bold>L ?G\<close>
 ]:
-  assumes F1: \<open>\<^bold>p\<^bold>r\<^bold>o\<^bold>c f1 \<lbrace> R \<longmapsto> R1\<heavy_comma> SYNTHESIS y \<Ztypecolon> \<bool> \<^bold>t\<^bold>h\<^bold>r\<^bold>o\<^bold>w\<^bold>s E1 \<rbrace>  \<^bold>@\<^bold>G\<^bold>O\<^bold>A\<^bold>L G\<close>
-    and   F2: \<open>\<^bold>p\<^bold>r\<^bold>o\<^bold>c f2 \<lbrace> R1 \<longmapsto> R2\<heavy_comma> SYNTHESIS x \<Ztypecolon> \<bool> \<^bold>t\<^bold>h\<^bold>r\<^bold>o\<^bold>w\<^bold>s E2 \<rbrace>  \<^bold>@\<^bold>G\<^bold>O\<^bold>A\<^bold>L G\<close>
+  assumes F1: \<open>\<^bold>p\<^bold>r\<^bold>o\<^bold>c f1 \<lbrace> R \<longmapsto> R1\<heavy_comma> SYNTHESIS y \<Ztypecolon> \<^bold>v\<^bold>a\<^bold>l \<bool> \<^bold>t\<^bold>h\<^bold>r\<^bold>o\<^bold>w\<^bold>s E1 \<rbrace>  \<^bold>@\<^bold>G\<^bold>O\<^bold>A\<^bold>L G\<close>
+    and   F2: \<open>\<^bold>p\<^bold>r\<^bold>o\<^bold>c f2 \<lbrace> R1 \<longmapsto> R2\<heavy_comma> SYNTHESIS x \<Ztypecolon> \<^bold>v\<^bold>a\<^bold>l \<bool> \<^bold>t\<^bold>h\<^bold>r\<^bold>o\<^bold>w\<^bold>s E2 \<rbrace>  \<^bold>@\<^bold>G\<^bold>O\<^bold>A\<^bold>L G\<close>
   goal G
   argument \<open>R\<close>
-  return   \<open>R2\<heavy_comma> SYNTHESIS VAL (x \<and> y) \<Ztypecolon> \<bool>\<close>
+  return   \<open>R2\<heavy_comma> SYNTHESIS (x \<and> y) \<Ztypecolon> \<^bold>v\<^bold>a\<^bold>l \<bool>\<close>
   throws   \<open>E1 + E2\<close>
-  \<medium_left_bracket> F1 \<rightarrow> y ;; F2 $y \<and> ;; \<medium_right_bracket>. .
+  \<medium_left_bracket> F1 \<rightarrow> yy ;; F2 $y \<and> ;; \<medium_right_bracket>. .
 
 paragraph \<open>Or\<close>
 
 lemma (in std) op_or[\<phi>overload \<or>]:
-  \<open>\<^bold>p\<^bold>r\<^bold>o\<^bold>c op_or \<lbrace> a \<Ztypecolon> \<bool>\<heavy_comma> b \<Ztypecolon> \<bool> \<longmapsto> a \<or> b \<Ztypecolon> \<bool> \<rbrace>\<close>
+  \<open>\<^bold>p\<^bold>r\<^bold>o\<^bold>c op_or vb va \<lbrace> a \<Ztypecolon> Val va \<bool>\<heavy_comma> b \<Ztypecolon> Val vb \<bool> \<longmapsto> a \<or> b \<Ztypecolon> \<^bold>v\<^bold>a\<^bold>l \<bool> \<rbrace>\<close>
   unfolding op_or_def
   by \<phi>reason
 
 proc [
     \<phi>reason on \<open>\<^bold>p\<^bold>r\<^bold>o\<^bold>c ?F \<lbrace> ?R \<longmapsto> ?R2\<heavy_comma> SYNTHESIS VAL (?x \<or> ?y) \<Ztypecolon> ?T \<^bold>t\<^bold>h\<^bold>r\<^bold>o\<^bold>w\<^bold>s ?E \<rbrace> \<^bold>@\<^bold>G\<^bold>O\<^bold>A\<^bold>L ?G\<close>
 ]:
-  assumes F1: \<open>\<^bold>p\<^bold>r\<^bold>o\<^bold>c f1 \<lbrace> R \<longmapsto> R1\<heavy_comma> y \<Ztypecolon> \<bool>\<heavy_comma> SYNTHESIS y \<Ztypecolon> \<bool> \<^bold>t\<^bold>h\<^bold>r\<^bold>o\<^bold>w\<^bold>s E1 \<rbrace>  \<^bold>@\<^bold>G\<^bold>O\<^bold>A\<^bold>L G\<close>
+  assumes F1: \<open>\<^bold>p\<^bold>r\<^bold>o\<^bold>c f1 \<lbrace> R \<longmapsto> R1\<heavy_comma> y \<Ztypecolon> \<^bold>v\<^bold>a\<^bold>l \<bool>\<heavy_comma> SYNTHESIS y \<Ztypecolon> \<^bold>v\<^bold>a\<^bold>l \<bool> \<^bold>t\<^bold>h\<^bold>r\<^bold>o\<^bold>w\<^bold>s E1 \<rbrace>  \<^bold>@\<^bold>G\<^bold>O\<^bold>A\<^bold>L G\<close>
     and   F2: \<open>\<^bold>p\<^bold>r\<^bold>o\<^bold>c f2 \<lbrace> R1 \<longmapsto> R2\<heavy_comma> SYNTHESIS x \<Ztypecolon> \<bool> \<^bold>t\<^bold>h\<^bold>r\<^bold>o\<^bold>w\<^bold>s E2 \<rbrace>  \<^bold>@\<^bold>G\<^bold>O\<^bold>A\<^bold>L G\<close>
   goal G
   argument \<open>R\<close>
@@ -235,7 +235,7 @@ proc [
 subsubsection \<open>Constant Integer\<close>
 
 lemma (in std) op_const_int_\<phi>app:
-  \<open>\<^bold>p\<^bold>r\<^bold>e\<^bold>m\<^bold>i\<^bold>s\<^bold>e n < 2^b \<Longrightarrow> \<^bold>p\<^bold>r\<^bold>o\<^bold>c op_const_int b n \<lbrace> Void \<longmapsto> n \<Ztypecolon> \<nat>[b] \<rbrace>\<close>
+  \<open>\<^bold>p\<^bold>r\<^bold>e\<^bold>m\<^bold>i\<^bold>s\<^bold>e n < 2^b \<Longrightarrow> \<^bold>p\<^bold>r\<^bold>o\<^bold>c op_const_int b n \<lbrace> Void \<longmapsto> n \<Ztypecolon> \<^bold>v\<^bold>a\<^bold>l \<nat>[b] \<rbrace>\<close>
   unfolding op_const_int_def Premise_def Synthesis_def
   by \<phi>reason
 
@@ -258,7 +258,7 @@ lemma (in std) [\<phi>reason
   using op_const_int_\<phi>app[THEN \<phi>frame, simplified] .
 
 lemma (in std) op_const_size_t:
-  \<open>\<^bold>p\<^bold>r\<^bold>o\<^bold>c op_const_size_t n \<lbrace> Void \<longmapsto> n \<Ztypecolon> Size \<rbrace>\<close>
+  \<open>\<^bold>p\<^bold>r\<^bold>o\<^bold>c op_const_size_t n \<lbrace> Void \<longmapsto> n \<Ztypecolon> \<^bold>v\<^bold>a\<^bold>l Size \<rbrace>\<close>
   unfolding op_const_size_t_def Premise_def
   by \<phi>reason
 
@@ -277,7 +277,7 @@ subsubsection \<open>Integer Arithmetic\<close>
 paragraph \<open>Addition\<close>
 
 lemma (in std) op_add[\<phi>overload +]:
-  \<open>\<^bold>p\<^bold>r\<^bold>e\<^bold>m\<^bold>i\<^bold>s\<^bold>e x + y < 2^b \<Longrightarrow> \<^bold>p\<^bold>r\<^bold>o\<^bold>c op_add b \<lbrace> x \<Ztypecolon> \<nat>[b]\<heavy_comma> y \<Ztypecolon> \<nat>[b] \<longmapsto> x + y \<Ztypecolon> \<nat>[b] \<rbrace>\<close>
+  \<open>\<^bold>p\<^bold>r\<^bold>e\<^bold>m\<^bold>i\<^bold>s\<^bold>e x + y < 2^b \<Longrightarrow> \<^bold>p\<^bold>r\<^bold>o\<^bold>c op_add b vy vx \<lbrace> x \<Ztypecolon> Val vx \<nat>[b]\<heavy_comma> y \<Ztypecolon> Val vy \<nat>[b] \<longmapsto> x + y \<Ztypecolon> \<^bold>v\<^bold>a\<^bold>l \<nat>[b] \<rbrace>\<close>
   unfolding op_add_def Premise_def
   by \<phi>reason
 
@@ -297,7 +297,7 @@ proc [
 paragraph \<open>Subtraction\<close>
 
 lemma (in std) op_sub[\<phi>overload -]:
-  \<open>\<^bold>p\<^bold>r\<^bold>e\<^bold>m\<^bold>i\<^bold>s\<^bold>e y \<le> x \<Longrightarrow> \<^bold>p\<^bold>r\<^bold>o\<^bold>c op_sub b \<lbrace> x \<Ztypecolon> \<nat>[b]\<heavy_comma> y \<Ztypecolon> \<nat>[b] \<longmapsto> x - y \<Ztypecolon> \<nat>[b] \<rbrace>\<close>
+  \<open>\<^bold>p\<^bold>r\<^bold>e\<^bold>m\<^bold>i\<^bold>s\<^bold>e y \<le> x \<Longrightarrow> \<^bold>p\<^bold>r\<^bold>o\<^bold>c op_sub b vy vx \<lbrace> x \<Ztypecolon> Val vx \<nat>[b]\<heavy_comma> y \<Ztypecolon> Val vy \<nat>[b] \<longmapsto> x - y \<Ztypecolon> \<^bold>v\<^bold>a\<^bold>l \<nat>[b] \<rbrace>\<close>
   unfolding op_sub_def Premise_def
   apply \<phi>reason
   apply (simp add: \<phi>expns)
@@ -319,7 +319,7 @@ proc [
 paragraph \<open>Division\<close>
 
 lemma (in std) op_udiv[\<phi>overload /]:
-  \<open>\<^bold>p\<^bold>r\<^bold>o\<^bold>c op_udiv b \<lbrace> x \<Ztypecolon> \<nat>[b]\<heavy_comma> y \<Ztypecolon> \<nat>[b] \<longmapsto> x div y \<Ztypecolon> \<nat>[b] \<rbrace>\<close>
+  \<open>\<^bold>p\<^bold>r\<^bold>o\<^bold>c op_udiv b vy vx \<lbrace> x \<Ztypecolon> Val vx \<nat>[b]\<heavy_comma> y \<Ztypecolon> Val vy \<nat>[b] \<longmapsto> x div y \<Ztypecolon> \<^bold>v\<^bold>a\<^bold>l \<nat>[b] \<rbrace>\<close>
   unfolding op_udiv_def Premise_def
   apply \<phi>reason apply (simp add: \<phi>expns)
   using div_le_dividend le_less_trans by blast
